<?xml version="1.0"?>


<!DOCTYPE rdf:RDF [
    <!ENTITY owl "http://www.w3.org/2002/07/owl#" >
    <!ENTITY xsd "http://www.w3.org/2001/XMLSchema#" >
    <!ENTITY rdfs "http://www.w3.org/2000/01/rdf-schema#" >
    <!ENTITY rdf "http://www.w3.org/1999/02/22-rdf-syntax-ns#" >
]>


<rdf:RDF xmlns="http://www.w3.org/ns/prov#"
     xml:base="http://www.w3.org/ns/prov"
     xmlns:rdfs="http://www.w3.org/2000/01/rdf-schema#"
     xmlns:owl="http://www.w3.org/2002/07/owl#"
     xmlns:xsd="http://www.w3.org/2001/XMLSchema#"
     xmlns:rdf="http://www.w3.org/1999/02/22-rdf-syntax-ns#">
    <owl:Ontology rdf:about="http://www.w3.org/ns/prov#">
        <rdfs:label xml:lang="en">PROV Ontology</rdfs:label>
        <rdfs:comment rdf:datatype="&xsd;string">0.2</rdfs:comment>
        <rdfs:comment xml:lang="en">This document is published by the Provenance Working Group (http://www.w3.org/2011/prov/wiki/Main_Page). 

If you wish to make comments regarding this document, please send them to public-prov-comments@w3.org (subscribe public-prov-comments-request@w3.org, archives http://lists.w3.org/Archives/Public/public-prov-comments/). All feedback is welcome.</rdfs:comment>
        <owl:versionIRI rdf:resource="http://www.w3.org/TR/2012/WD-prov-o-2012MMDD"/>
        <rdfs:seeAlso rdf:resource="http://www.w3.org/TR/prov#"/>
        <rdfs:seeAlso rdf:resource="http://www.w3.org/TR/prov-o/"/>
    </owl:Ontology>
    


    <!-- 
    ///////////////////////////////////////////////////////////////////////////////////////
    //
    // Annotation properties
    //
    ///////////////////////////////////////////////////////////////////////////////////////
     -->

    <owl:AnnotationProperty rdf:about="http://www.w3.org/ns/prov#unqualifiedForm">
        <rdfs:comment xml:lang="en">Classes and properties used to qualify relationships are annotated with prov:unqualifiedForm to indicate the property used to assert an unqualified provenance relation.</rdfs:comment>
        <rdfs:subPropertyOf rdf:resource="&rdfs;seeAlso"/>
    </owl:AnnotationProperty>
    <owl:AnnotationProperty rdf:about="http://www.w3.org/ns/prov#prov-n">
        <rdfs:comment xml:lang="en">A reference to the principal section of the PROV-M document that describes this concept.</rdfs:comment>
        <rdfs:subPropertyOf rdf:resource="&rdfs;seeAlso"/>
    </owl:AnnotationProperty>
    <owl:AnnotationProperty rdf:about="http://www.w3.org/ns/prov#sharesDefinitionWith">
        <rdfs:subPropertyOf rdf:resource="&rdfs;seeAlso"/>
    </owl:AnnotationProperty>
    <owl:AnnotationProperty rdf:about="http://www.w3.org/ns/prov#prov-dm">
        <rdfs:comment xml:lang="en">A reference to the principal section of the PROV-DM document that describes this concept.</rdfs:comment>
        <rdfs:subPropertyOf rdf:resource="&rdfs;seeAlso"/>
    </owl:AnnotationProperty>
    <owl:AnnotationProperty rdf:about="http://www.w3.org/ns/prov#definition">
        <rdfs:comment xml:lang="en">A definition quoted from PROV-DM or PROV-CONSTRAINTS that describes the concept expressed with this OWL term.</rdfs:comment>
    </owl:AnnotationProperty>
    <owl:AnnotationProperty rdf:about="http://www.w3.org/ns/prov#editorialNote">
        <rdfs:comment xml:lang="en">A note by the OWL development team about how this term expresses the PROV-DM concept, or how it should be used in context of semantic web or linked data.</rdfs:comment>
    </owl:AnnotationProperty>
    <owl:AnnotationProperty rdf:about="&rdfs;label">
        <rdfs:comment xml:lang="en"></rdfs:comment>
    </owl:AnnotationProperty>
    <owl:AnnotationProperty rdf:about="http://www.w3.org/ns/prov#inverse">
        <rdfs:comment xml:lang="en">PROV-O does not define all property inverses. The directionalities defined in PROV-O should be given preference over those not defined. However, if users wish to name the inverse of a PROV-O property, the local name given by prov:inverse should be used.</rdfs:comment>
        <rdfs:seeAlso rdf:resource="http://www.w3.org/TR/prov-o/#names-of-inverse-properties"/>
    </owl:AnnotationProperty>
    <owl:AnnotationProperty rdf:about="&rdfs;comment">
        <rdfs:comment xml:lang="en"></rdfs:comment>
    </owl:AnnotationProperty>
    <owl:AnnotationProperty rdf:about="&rdfs;seeAlso">
        <rdfs:comment xml:lang="en"></rdfs:comment>
    </owl:AnnotationProperty>
    <owl:AnnotationProperty rdf:about="&owl;versionInfo"/>
    <owl:AnnotationProperty rdf:about="http://www.w3.org/ns/prov#category">
        <rdfs:comment xml:lang="en">Classify prov-o terms into three categories, including &#39;starting-point&#39;, &#39;qualifed&#39;, and &#39;extended&#39;. This classification is used by the prov-o html document to gently introduce prov-o terms to its users. </rdfs:comment>
    </owl:AnnotationProperty>
    <owl:AnnotationProperty rdf:about="http://www.w3.org/ns/prov#prov-dm-constraints">
        <rdfs:comment xml:lang="en">A reference to the principal section of the PROV-CONSTRAINTS document that describes this concept.</rdfs:comment>
        <rdfs:subPropertyOf rdf:resource="&rdfs;seeAlso"/>
    </owl:AnnotationProperty>
    <owl:AnnotationProperty rdf:about="&rdfs;isDefinedBy"/>
    <owl:AnnotationProperty rdf:about="http://www.w3.org/ns/prov#editorsDefinition">
        <rdfs:comment xml:lang="en">When the prov-o term does not have a definition drawn from prov-dm, and the prov-o editor provides one.</rdfs:comment>
        <rdfs:subPropertyOf rdf:resource="http://www.w3.org/ns/prov#definition"/>
    </owl:AnnotationProperty>
    <owl:AnnotationProperty rdf:about="http://www.w3.org/ns/prov#prov-aq">
        <rdfs:subPropertyOf rdf:resource="&rdfs;seeAlso"/>
    </owl:AnnotationProperty>
    <owl:AnnotationProperty rdf:about="http://www.w3.org/ns/prov#component">
        <rdfs:comment xml:lang="en">Classify prov-o terms into six components according to prov-dm, including &#39;agents-responsibility&#39;, &#39;alternate&#39;, &#39;annotations&#39;, &#39;collections&#39;, &#39;derivations&#39;, and &#39;entities-activities&#39;. This classification is used so that readers of prov-o specification can find its correspondence with the prov-dm specification.</rdfs:comment>
    </owl:AnnotationProperty>
    <owl:AnnotationProperty rdf:about="http://www.w3.org/ns/prov#qualifiedForm">
        <rdfs:comment xml:lang="en">This annotation property links a prov:involved subproperty with a prov:Involved subclass. This indicates that the property can be qualified by using prov:qualified. 

Example:
    prov:wasGeneratedBy prov:qualifiedForm prov:Generation .

Then this unqualified assertion:
    :entity1 prov:wasGeneratedBy :activity1 .

can be qualified by adding:
   :entity1 prov:qualified :entity1Gen .
   :entity1Gen a prov:Generation;
       prov:activity :activity1 ;
       :customValue 1337 .

Note how the range of the unqualified property is mirrored by the prov:activity or prov:entity on the involvement class.</rdfs:comment>
        <rdfs:subPropertyOf rdf:resource="&rdfs;seeAlso"/>
    </owl:AnnotationProperty>
    <owl:AnnotationProperty rdf:about="http://www.w3.org/ns/prov#todo"/>
    


    <!-- 
    ///////////////////////////////////////////////////////////////////////////////////////
    //
    // Object Properties
    //
    ///////////////////////////////////////////////////////////////////////////////////////
     -->

    


    <!-- http://www.w3.org/2002/07/owl#topObjectProperty -->

    <owl:ObjectProperty rdf:about="&owl;topObjectProperty"/>
    


    <!-- http://www.w3.org/ns/prov#actedOnBehalfOf -->

    <owl:ObjectProperty rdf:about="http://www.w3.org/ns/prov#actedOnBehalfOf">
        <rdfs:comment xml:lang="en">An object property to express the accountability of an agent towards another agent. The subordinate agent acted on behalf of the responsible agent in an actual activity. </rdfs:comment>
        <category>starting-point</category>
        <inverse>hadDelegate</inverse>
        <component>agents-responsibility</component>
        <rdfs:domain rdf:resource="http://www.w3.org/ns/prov#Agent"/>
        <rdfs:range rdf:resource="http://www.w3.org/ns/prov#Agent"/>
        <qualifiedForm rdf:resource="http://www.w3.org/ns/prov#Delegation"/>
        <rdfs:subPropertyOf rdf:resource="http://www.w3.org/ns/prov#involved"/>
        <qualifiedForm rdf:resource="http://www.w3.org/ns/prov#qualifiedDelegation"/>
        <owl:propertyChainAxiom rdf:parseType="Collection">
            <rdf:Description rdf:about="http://www.w3.org/ns/prov#qualifiedDelegation"/>
            <rdf:Description rdf:about="http://www.w3.org/ns/prov#agent"/>
        </owl:propertyChainAxiom>
    </owl:ObjectProperty>
    


    <!-- http://www.w3.org/ns/prov#activity -->

    <owl:ObjectProperty rdf:about="http://www.w3.org/ns/prov#activity">
        <rdf:type rdf:resource="&owl;FunctionalProperty"/>
        <rdfs:comment xml:lang="en">The property used by an prov:ActivityInvolvement to cite the prov:Activity that was involved with either an Activity or Entity. It can be used to refer to the activity involved in generating an entity, informing another activity, or starting another activity.</rdfs:comment>
        <editorialNote xml:lang="en">This property behaves in spirit like rdf:object; it references the object of a prov:involved triple.</editorialNote>
        <inverse>activityOfInvolvement</inverse>
        <category>qualified</category>
        <rdfs:range rdf:resource="http://www.w3.org/ns/prov#Activity"/>
        <sharesDefinitionWith rdf:resource="http://www.w3.org/ns/prov#ActivityInvolvement"/>
        <rdfs:domain rdf:resource="http://www.w3.org/ns/prov#ActivityInvolvement"/>
        <rdfs:subPropertyOf rdf:resource="http://www.w3.org/ns/prov#involvee"/>
    </owl:ObjectProperty>
    


    <!-- http://www.w3.org/ns/prov#agent -->

    <owl:ObjectProperty rdf:about="http://www.w3.org/ns/prov#agent">
        <rdf:type rdf:resource="&owl;FunctionalProperty"/>
        <component>alternate</component>
        <inverse>agentOfInvolvement</inverse>
        <rdfs:comment xml:lang="en">The property used by a prov:AgentInvolvement to cite the Agent that was prov:involved with either an Activity or Entity. It can be used to express the agent involved in being responsible for an activity, being attributed to an entity, starting or ending an activity, or being responsible for another subordinate agent in an activity.</rdfs:comment>
        <editorialNote xml:lang="en">This property behaves in spirit like rdf:object; it references the object of a prov:involved triple.</editorialNote>
        <category>qualified</category>
        <rdfs:range rdf:resource="http://www.w3.org/ns/prov#Agent"/>
        <rdfs:domain rdf:resource="http://www.w3.org/ns/prov#AgentInvolvement"/>
        <sharesDefinitionWith rdf:resource="http://www.w3.org/ns/prov#AgentInvolvement"/>
        <rdfs:subPropertyOf rdf:resource="http://www.w3.org/ns/prov#involvee"/>
    </owl:ObjectProperty>
    


    <!-- http://www.w3.org/ns/prov#alternateOf -->

    <owl:ObjectProperty rdf:about="http://www.w3.org/ns/prov#alternateOf">
        <rdf:type rdf:resource="&owl;ReflexiveProperty"/>
        <rdf:type rdf:resource="&owl;SymmetricProperty"/>
        <rdf:type rdf:resource="&owl;TransitiveProperty"/>
        <prov-dm-constraints>http://dvcs.w3.org/hg/prov/raw-file/default/model/prov-dm-constraints.html#term-Alternate</prov-dm-constraints>
        <category>expanded</category>
        <component>alternate</component>
        <prov-n>http://dvcs.w3.org/hg/prov/raw-file/default/model/prov-n.html#expression-alternate</prov-n>
        <prov-dm>http://dvcs.w3.org/hg/prov/raw-file/default/model/prov-dm.html#term-alternate</prov-dm>
        <inverse>alternateOf</inverse>
        <definition xml:lang="en">An entity is alternate of another if they are both a specialization of some common entity. The common entity does not need to be identified.</definition>
        <rdfs:comment xml:lang="en">An entity is alternate of another if they are both a specialization of some common entity. The common entity does not need to be identified.</rdfs:comment>
        <rdfs:subPropertyOf rdf:resource="&owl;topObjectProperty"/>
        <rdfs:domain rdf:resource="http://www.w3.org/ns/prov#Entity"/>
        <rdfs:range rdf:resource="http://www.w3.org/ns/prov#Entity"/>
        <rdfs:seeAlso rdf:resource="http://www.w3.org/ns/prov#specializationOf"/>
    </owl:ObjectProperty>
    


    <!-- http://www.w3.org/ns/prov#atLocation -->

    <owl:ObjectProperty rdf:about="http://www.w3.org/ns/prov#atLocation">
        <rdf:type rdf:resource="&owl;AsymmetricProperty"/>
        <rdf:type rdf:resource="&owl;IrreflexiveProperty"/>
        <editorialNote>This property is not functional because the many values could be at a variety of granularies (In this building, in this room, in that chair).</editorialNote>
        <rdfs:comment xml:lang="en">The Location of any resource.</rdfs:comment>
        <inverse>locationOf</inverse>
        <category>expanded</category>
        <editorialNote>The naming of prov:atLocation parallels prov:atTime, and is not named prov:hadLocation to avoid conflicting with the convention that prov:had* properties are used on prov:Involvement classes.</editorialNote>
        <sharesDefinitionWith rdf:resource="http://www.w3.org/ns/prov#Location"/>
        <rdfs:range rdf:resource="http://www.w3.org/ns/prov#Location"/>
    </owl:ObjectProperty>
    


    <!-- http://www.w3.org/ns/prov#contextualized -->

    <owl:ObjectProperty rdf:about="http://www.w3.org/ns/prov#contextualized">
        <category>expanded</category>
        <inverse>hasContextualization</inverse>
        <sharesDefinitionWith rdf:resource="http://www.w3.org/ns/prov#ContextualizedEntity"/>
        <rdfs:domain rdf:resource="http://www.w3.org/ns/prov#ContextualizedEntity"/>
        <rdfs:subPropertyOf rdf:resource="http://www.w3.org/ns/prov#specializationOf"/>
    </owl:ObjectProperty>
    


    <!-- http://www.w3.org/ns/prov#derivedByInsertionFrom -->

    <owl:ObjectProperty rdf:about="http://www.w3.org/ns/prov#derivedByInsertionFrom">
        <rdfs:comment xml:lang="en">The dictionary was derived from the other by insertion. prov:qualifiedInsertion shows details of the insertion, in particular the inserted key-value pairs.</rdfs:comment>
        <inverse>hadDerivationByInsertion</inverse>
        <component>collections</component>
        <category>collections</category>
        <rdfs:range rdf:resource="http://www.w3.org/ns/prov#Dictionary"/>
        <rdfs:domain rdf:resource="http://www.w3.org/ns/prov#Dictionary"/>
        <qualifiedForm rdf:resource="http://www.w3.org/ns/prov#Insertion"/>
        <qualifiedForm rdf:resource="http://www.w3.org/ns/prov#qualifiedInsertion"/>
        <rdfs:subPropertyOf rdf:resource="http://www.w3.org/ns/prov#wasDerivedFrom"/>
        <owl:propertyChainAxiom rdf:parseType="Collection">
            <rdf:Description rdf:about="http://www.w3.org/ns/prov#qualifiedInsertion"/>
            <rdf:Description rdf:about="http://www.w3.org/ns/prov#dictionary"/>
        </owl:propertyChainAxiom>
    </owl:ObjectProperty>
    <owl:Axiom>
        <rdfs:comment>Insertion is a form of derivation (see http://www.w3.org/TR/prov-dm/#term-dictionary-insertion) that transforms a dictionary into another, by insertion of one or more key-entity pairs. </rdfs:comment>
        <owl:annotatedProperty rdf:resource="&rdfs;subPropertyOf"/>
        <owl:annotatedSource rdf:resource="http://www.w3.org/ns/prov#derivedByInsertionFrom"/>
        <owl:annotatedTarget rdf:resource="http://www.w3.org/ns/prov#wasDerivedFrom"/>
    </owl:Axiom>
    


    <!-- http://www.w3.org/ns/prov#derivedByRemovalFrom -->

    <owl:ObjectProperty rdf:about="http://www.w3.org/ns/prov#derivedByRemovalFrom">
        <rdfs:comment xml:lang="en">The dictionary was derived from the other by removal. prov:qualifiedRemoval shows details of the removal, in particular the removed key-value pairs.</rdfs:comment>
        <component>collections</component>
        <category>collections</category>
        <inverse>hadDerivationByRemoval</inverse>
        <rdfs:range rdf:resource="http://www.w3.org/ns/prov#Dictionary"/>
        <rdfs:domain rdf:resource="http://www.w3.org/ns/prov#Dictionary"/>
        <qualifiedForm rdf:resource="http://www.w3.org/ns/prov#Removal"/>
        <qualifiedForm rdf:resource="http://www.w3.org/ns/prov#qualifiedRemoval"/>
        <rdfs:subPropertyOf rdf:resource="http://www.w3.org/ns/prov#wasDerivedFrom"/>
        <owl:propertyChainAxiom rdf:parseType="Collection">
            <rdf:Description rdf:about="http://www.w3.org/ns/prov#qualifiedRemoval"/>
            <rdf:Description rdf:about="http://www.w3.org/ns/prov#dictionary"/>
        </owl:propertyChainAxiom>
    </owl:ObjectProperty>
    <owl:Axiom>
        <rdfs:comment>Removal is a form of derivation (see http://www.w3.org/TR/prov-dm/#term-dictionary-removal) that transforms a dictionary into another, by removing one or more key-entity pairs. </rdfs:comment>
        <owl:annotatedProperty rdf:resource="&rdfs;subPropertyOf"/>
        <owl:annotatedSource rdf:resource="http://www.w3.org/ns/prov#derivedByRemovalFrom"/>
        <owl:annotatedTarget rdf:resource="http://www.w3.org/ns/prov#wasDerivedFrom"/>
    </owl:Axiom>
    


    <!-- http://www.w3.org/ns/prov#dictionary -->

    <owl:ObjectProperty rdf:about="http://www.w3.org/ns/prov#dictionary">
        <inverse>dictionaryOfInvolvement</inverse>
        <rdfs:comment xml:lang="en">The property used by a prov:DictionaryInvolvement to cite the prov:Dictionary that was prov:involved in insertion or removal of elements of a collection. </rdfs:comment>
        <editorialNote xml:lang="en">This property behaves in spirit like rdf:object; it references the object of a prov:involved triple.</editorialNote>
        <component>collections</component>
        <category>collections</category>
        <rdfs:range rdf:resource="http://www.w3.org/ns/prov#Dictionary"/>
        <rdfs:domain rdf:resource="http://www.w3.org/ns/prov#DictionaryInvolvement"/>
        <sharesDefinitionWith rdf:resource="http://www.w3.org/ns/prov#DictionaryInvolvement"/>
        <rdfs:subPropertyOf rdf:resource="http://www.w3.org/ns/prov#involvee"/>
    </owl:ObjectProperty>
    


    <!-- http://www.w3.org/ns/prov#entity -->

    <owl:ObjectProperty rdf:about="http://www.w3.org/ns/prov#entity">
        <rdf:type rdf:resource="&owl;FunctionalProperty"/>
        <rdfs:comment xml:lang="en">The property used by an prov:EntityInvolvement to cite the Entity that was prov:involved with either an Activity or Entity. It can be used to refer to the entity involved in deriving another entity, being quoted or revised from, being the source of another entity, or being used in an activity. </rdfs:comment>
        <inverse>entityOfInvolvement</inverse>
        <editorialNote xml:lang="en">This property behaves in spirit like rdf:object; it references the object of a prov:involved triple.</editorialNote>
        <category>qualified</category>
        <rdfs:range rdf:resource="http://www.w3.org/ns/prov#Entity"/>
        <sharesDefinitionWith rdf:resource="http://www.w3.org/ns/prov#EntityInvolvement"/>
        <rdfs:domain rdf:resource="http://www.w3.org/ns/prov#EntityInvolvement"/>
        <rdfs:subPropertyOf rdf:resource="http://www.w3.org/ns/prov#involvee"/>
    </owl:ObjectProperty>
    


    <!-- http://www.w3.org/ns/prov#generated -->

    <owl:ObjectProperty rdf:about="http://www.w3.org/ns/prov#generated">
        <component>entities-activities</component>
        <inverse>wasGeneratedBy</inverse>
        <category>expanded</category>
        <rdfs:comment>This inverse of prov:wasGeneratedBy is defined so that Activities being described can reference their generated outputs directly without needing to &#39;stop&#39; and start describing the Entity. This helps &#39;Activity-centric&#39; modeling as opposed to &#39;Entity-centric&#39; modeling.</rdfs:comment>
        <rdfs:domain rdf:resource="http://www.w3.org/ns/prov#Activity"/>
        <rdfs:range rdf:resource="http://www.w3.org/ns/prov#Entity"/>
        <sharesDefinitionWith rdf:resource="http://www.w3.org/ns/prov#Generation"/>
        <rdfs:subPropertyOf rdf:resource="http://www.w3.org/ns/prov#involved"/>
        <owl:inverseOf rdf:resource="http://www.w3.org/ns/prov#wasGeneratedBy"/>
    </owl:ObjectProperty>
    


    <!-- http://www.w3.org/ns/prov#hadActivity -->

    <owl:ObjectProperty rdf:about="http://www.w3.org/ns/prov#hadActivity">
        <rdf:type rdf:resource="&owl;FunctionalProperty"/>
        <component>derivations</component>
        <category>qualified</category>
        <inverse>wasActivityOfInvolvement</inverse>
        <editorialNote>The multiple rdfs:domain assertions are intended. One is simpler and works for OWL-RL, the union is more specific but is not recognized by OWL-RL.</editorialNote>
        <rdfs:comment xml:lang="en">The _optional_ Activity of an Involvement, which used, generated, invalidated, or was the responsibility of some Entity. This property is _not_ used by ActivityInvolvement (use prov:activity instead).</rdfs:comment>
        <rdfs:range rdf:resource="http://www.w3.org/ns/prov#Activity"/>
        <sharesDefinitionWith rdf:resource="http://www.w3.org/ns/prov#Activity"/>
        <rdfs:domain rdf:resource="http://www.w3.org/ns/prov#Involvement"/>
        <rdfs:domain>
            <owl:Class>
                <owl:unionOf rdf:parseType="Collection">
                    <rdf:Description rdf:about="http://www.w3.org/ns/prov#Delegation"/>
                    <rdf:Description rdf:about="http://www.w3.org/ns/prov#Derivation"/>
                    <rdf:Description rdf:about="http://www.w3.org/ns/prov#Start"/>
                </owl:unionOf>
            </owl:Class>
        </rdfs:domain>
    </owl:ObjectProperty>
    


    <!-- http://www.w3.org/ns/prov#hadGeneration -->

    <owl:ObjectProperty rdf:about="http://www.w3.org/ns/prov#hadGeneration">
        <rdf:type rdf:resource="&owl;FunctionalProperty"/>
        <inverse>generatedAsDerivation</inverse>
        <category>qualified</category>
        <rdfs:comment xml:lang="en">The _optional_ Generation involved in an Entity&#39;s Derivation.</rdfs:comment>
        <component>derivations</component>
        <rdfs:domain rdf:resource="http://www.w3.org/ns/prov#Derivation"/>
        <sharesDefinitionWith rdf:resource="http://www.w3.org/ns/prov#Generation"/>
        <rdfs:range rdf:resource="http://www.w3.org/ns/prov#Generation"/>
    </owl:ObjectProperty>
    


    <!-- http://www.w3.org/ns/prov#hadMember -->

    <owl:ObjectProperty rdf:about="http://www.w3.org/ns/prov#hadMember">
        <component>collections</component>
        <prov-dm>http://dvcs.w3.org/hg/prov/raw-file/default/model/prov-dm.html#term-collection</prov-dm>
        <category>collections</category>
        <inverse>wasMemberOf</inverse>
        <sharesDefinitionWith rdf:resource="http://www.w3.org/ns/prov#Collection"/>
        <rdfs:domain rdf:resource="http://www.w3.org/ns/prov#Collection"/>
        <rdfs:range rdf:resource="http://www.w3.org/ns/prov#Entity"/>
        <owl:propertyChainAxiom rdf:parseType="Collection">
            <rdf:Description rdf:about="http://www.w3.org/ns/prov#qualifiedMembership"/>
            <rdf:Description rdf:about="http://www.w3.org/ns/prov#pair"/>
        </owl:propertyChainAxiom>
    </owl:ObjectProperty>
    <owl:Axiom>
        <prov-dm>http://dvcs.w3.org/hg/prov/raw-file/default/model/prov-dm.html#term-collection</prov-dm>
        <rdfs:comment xml:lang="en">A collection is an entity that provides a structure to some constituents, which are themselves entities. These constituents are said to be member of the collections.</rdfs:comment>
        <owl:annotatedProperty rdf:resource="&rdfs;range"/>
        <owl:annotatedTarget rdf:resource="http://www.w3.org/ns/prov#Entity"/>
        <owl:annotatedSource rdf:resource="http://www.w3.org/ns/prov#hadMember"/>
    </owl:Axiom>
    


    <!-- http://www.w3.org/ns/prov#hadPlan -->

    <owl:ObjectProperty rdf:about="http://www.w3.org/ns/prov#hadPlan">
        <rdf:type rdf:resource="&owl;AsymmetricProperty"/>
        <rdf:type rdf:resource="&owl;FunctionalProperty"/>
        <rdf:type rdf:resource="&owl;IrreflexiveProperty"/>
        <category>qualified</category>
        <component>agents-responsibility</component>
        <inverse>wasPlanOf</inverse>
        <rdfs:comment xml:lang="en">The _optional_ Plan adopted by an Agent in Association with some Activity. Plan specifications are out of the scope of this specification.</rdfs:comment>
        <rdfs:domain rdf:resource="http://www.w3.org/ns/prov#Association"/>
        <sharesDefinitionWith rdf:resource="http://www.w3.org/ns/prov#Plan"/>
        <rdfs:range rdf:resource="http://www.w3.org/ns/prov#Plan"/>
    </owl:ObjectProperty>
    


    <!-- http://www.w3.org/ns/prov#hadPrimarySource -->

    <owl:ObjectProperty rdf:about="http://www.w3.org/ns/prov#hadPrimarySource">
        <component>derivations</component>
        <rdfs:comment xml:lang="en">An original source refers to the source material that is closest to the person, information, period, or idea being studied. An original source relation is a particular case of derivation that aims to give credit to the source that originated some information.</rdfs:comment>
        <category>expanded</category>
        <inverse>wasPrimarySourceOf</inverse>
        <rdfs:range rdf:resource="http://www.w3.org/ns/prov#Entity"/>
        <rdfs:domain rdf:resource="http://www.w3.org/ns/prov#Entity"/>
        <qualifiedForm rdf:resource="http://www.w3.org/ns/prov#Source"/>
        <qualifiedForm rdf:resource="http://www.w3.org/ns/prov#qualifiedSource"/>
        <rdfs:subPropertyOf rdf:resource="http://www.w3.org/ns/prov#wasDerivedFrom"/>
        <owl:propertyChainAxiom rdf:parseType="Collection">
            <rdf:Description rdf:about="http://www.w3.org/ns/prov#qualifiedSource"/>
            <rdf:Description rdf:about="http://www.w3.org/ns/prov#entity"/>
        </owl:propertyChainAxiom>
    </owl:ObjectProperty>
    <owl:Axiom>
        <rdfs:comment>hadOriginalSource property is a particular case of wasDerivedFrom (see http://www.w3.org/TR/prov-dm/#term-original-source) that aims to give credit to the source that originated some information.</rdfs:comment>
        <owl:annotatedProperty rdf:resource="&rdfs;subPropertyOf"/>
        <owl:annotatedSource rdf:resource="http://www.w3.org/ns/prov#hadPrimarySource"/>
        <owl:annotatedTarget rdf:resource="http://www.w3.org/ns/prov#wasDerivedFrom"/>
    </owl:Axiom>
    


    <!-- http://www.w3.org/ns/prov#hadRole -->

    <owl:ObjectProperty rdf:about="http://www.w3.org/ns/prov#hadRole">
        <rdf:type rdf:resource="&owl;IrreflexiveProperty"/>
        <component>agents-responsibility</component>
        <rdfs:comment xml:lang="en">The _optional_ Role that an Entity assumes in the context of an Activity. For example, :baking prov:used :spoon; prov:qualified [ a prov:Usage; prov:entity :spoon; prov:hadRole roles:mixing_implement ].</rdfs:comment>
        <definition>prov:hadRole references the Role (i.e. the function of an entity with respect to an activity), in the context of a usage, generation, association, start, and end.</definition>
        <category>qualified</category>
        <inverse>wasRoleIn</inverse>
        <rdfs:domain rdf:resource="http://www.w3.org/ns/prov#Involvement"/>
        <sharesDefinitionWith rdf:resource="http://www.w3.org/ns/prov#Role"/>
        <rdfs:range rdf:resource="http://www.w3.org/ns/prov#Role"/>
        <rdfs:domain>
            <owl:Class>
                <owl:unionOf rdf:parseType="Collection">
                    <rdf:Description rdf:about="http://www.w3.org/ns/prov#Association"/>
                    <rdf:Description rdf:about="http://www.w3.org/ns/prov#End"/>
                    <rdf:Description rdf:about="http://www.w3.org/ns/prov#Generation"/>
                    <rdf:Description rdf:about="http://www.w3.org/ns/prov#Invalidation"/>
                    <rdf:Description rdf:about="http://www.w3.org/ns/prov#Start"/>
                    <rdf:Description rdf:about="http://www.w3.org/ns/prov#Usage"/>
                </owl:unionOf>
            </owl:Class>
        </rdfs:domain>
    </owl:ObjectProperty>
    


    <!-- http://www.w3.org/ns/prov#hadUsage -->

    <owl:ObjectProperty rdf:about="http://www.w3.org/ns/prov#hadUsage">
        <rdf:type rdf:resource="&owl;FunctionalProperty"/>
        <category>qualified</category>
        <rdfs:comment xml:lang="en">The _optional_ Usage involved in an Entity&#39;s Derivation.</rdfs:comment>
        <inverse>wasUsedInDerivation</inverse>
        <component>derivations</component>
        <rdfs:domain rdf:resource="http://www.w3.org/ns/prov#Derivation"/>
        <rdfs:range rdf:resource="http://www.w3.org/ns/prov#Usage"/>
        <sharesDefinitionWith rdf:resource="http://www.w3.org/ns/prov#Usage"/>
    </owl:ObjectProperty>
    


    <!-- http://www.w3.org/ns/prov#hasAnchor -->

    <owl:ObjectProperty rdf:about="http://www.w3.org/ns/prov#hasAnchor">
        <inverse>anchorOf</inverse>
        <rdfs:comment xml:lang="en">Indicates anchor URI for a potentially dynamic resource instance.</rdfs:comment>
        <category>access-and-query</category>
        <prov-aq>http://dvcs.w3.org/hg/prov/raw-file/tip/paq/prov-aq.html#todo</prov-aq>
    </owl:ObjectProperty>
    


    <!-- http://www.w3.org/ns/prov#hasProvenance -->

    <owl:ObjectProperty rdf:about="http://www.w3.org/ns/prov#hasProvenance">
        <prov-aq>http://dvcs.w3.org/hg/prov/raw-file/tip/paq/prov-aq.html#todo</prov-aq>
        <inverse>provenanceOf</inverse>
        <rdfs:comment xml:lang="en">Relates a resource to its provenance.</rdfs:comment>
        <category>access-and-query</category>
    </owl:ObjectProperty>
    


    <!-- http://www.w3.org/ns/prov#hasProvenanceService -->

    <owl:ObjectProperty rdf:about="http://www.w3.org/ns/prov#hasProvenanceService">
        <rdfs:comment xml:lang="en">Relates a resource to a provenance service.</rdfs:comment>
        <category>access-and-query</category>
        <prov-aq>http://dvcs.w3.org/hg/prov/raw-file/tip/paq/prov-aq.html#todo</prov-aq>
        <inverse>provenanceAnchorOf</inverse>
    </owl:ObjectProperty>
    


    <!-- http://www.w3.org/ns/prov#inContext -->

    <owl:ObjectProperty rdf:about="http://www.w3.org/ns/prov#inContext">
        <category>expanded</category>
        <inverse>contextOf</inverse>
        <sharesDefinitionWith rdf:resource="http://www.w3.org/ns/prov#ContextualizedEntity"/>
        <rdfs:domain rdf:resource="http://www.w3.org/ns/prov#ContextualizedEntity"/>
    </owl:ObjectProperty>
    


    <!-- http://www.w3.org/ns/prov#inserted -->

    <owl:ObjectProperty rdf:about="http://www.w3.org/ns/prov#inserted">
        <rdfs:comment xml:lang="en">An object property to refer to the prov:KeyValuePair inserted into a prov:Dictionary.</rdfs:comment>
        <inverse>wasInsertedBy</inverse>
        <component>collections</component>
        <category>collections</category>
        <rdfs:domain rdf:resource="http://www.w3.org/ns/prov#Insertion"/>
        <sharesDefinitionWith rdf:resource="http://www.w3.org/ns/prov#Insertion"/>
        <rdfs:range rdf:resource="http://www.w3.org/ns/prov#KeyValuePair"/>
    </owl:ObjectProperty>
    


    <!-- http://www.w3.org/ns/prov#involved -->

    <owl:ObjectProperty rdf:about="http://www.w3.org/ns/prov#involved">
        <category>qualified</category>
        <inverse>wasInvolvedWith</inverse>
        <editorsDefinition xml:lang="en">The broadest provenance relation between two resources, prov:involved is the superproperty of all unqualified binary relations among any two Activities, Entities, or Agents (or anything else). A more specific property should be favored of prov:involved.</editorsDefinition>
        <editorialNote xml:lang="en">The relation the sub-properties of prov:involved can also be specified in more detail using the qualification pattern. For example, the binary relation :baking prov:used :spoon can be qualified by asserting :baking prov:qualifiedUsage [ a prov:Usage; prov:entity :baking; :foo :bar; prov:atLocation :kitchen ] .

Subproperties of prov:involved may also be asserted directly without being qualified.

prov:involved should not be used without also using one of its subproperties. 

</editorialNote>
    </owl:ObjectProperty>
    


    <!-- http://www.w3.org/ns/prov#involvee -->

    <owl:ObjectProperty rdf:about="http://www.w3.org/ns/prov#involvee">
        <inverse>involvement</inverse>
        <category>qualified</category>
        <rdfs:comment>Subproperties of prov:involvee are used to cite the object of an unqualified PROV-O triple whose predicate is a subproperty of prov:involved (e.g. prov:used, prov:wasGeneratedBy). prov:involvee is used much like rdf:object is used.</rdfs:comment>
        <editorsDefinition xml:lang="en">The rdf:object of the (binary) prov:involved relation (triple) that this Involvement is qualifying (reifying) for further description (as an n-ary relation).</editorsDefinition>
        <rdfs:domain rdf:resource="http://www.w3.org/ns/prov#Involvement"/>
    </owl:ObjectProperty>
    


    <!-- http://www.w3.org/ns/prov#pair -->

    <owl:ObjectProperty rdf:about="http://www.w3.org/ns/prov#pair">
        <component>collections</component>
        <category>collections</category>
        <rdfs:comment xml:lang="en">A membership can have multiple members.</rdfs:comment>
        <editorsDefinition xml:lang="en">The KeyValuePair(s) whose membership is being qualified by this instance of prov:Membership.</editorsDefinition>
        <editorialNote xml:lang="en">This property behaves in spirit like rdf:object; it references the object of a prov:involved triple.</editorialNote>
        <inverse>inMembership</inverse>
        <rdfs:range rdf:resource="http://www.w3.org/ns/prov#KeyValuePair"/>
        <rdfs:domain rdf:resource="http://www.w3.org/ns/prov#Membership"/>
        <rdfs:subPropertyOf rdf:resource="http://www.w3.org/ns/prov#involvee"/>
    </owl:ObjectProperty>
    


    <!-- http://www.w3.org/ns/prov#pairValue -->

    <owl:ObjectProperty rdf:about="http://www.w3.org/ns/prov#pairValue">
        <rdf:type rdf:resource="&owl;FunctionalProperty"/>
        <editorsDefinition xml:lang="en">The Entity value of a KeyValuePair, which may go into a prov:Dictionary under the key specified by prov:pairKey.</editorsDefinition>
        <rdfs:comment xml:lang="en">The value of a KeyValuePair. See also prov:pairKey.</rdfs:comment>
        <category>collections</category>
        <inverse>valueOf</inverse>
        <component>collections</component>
        <rdfs:range rdf:resource="http://www.w3.org/ns/prov#Entity"/>
        <rdfs:domain rdf:resource="http://www.w3.org/ns/prov#KeyValuePair"/>
    </owl:ObjectProperty>
    


    <!-- http://www.w3.org/ns/prov#qualifiedAssociation -->

    <owl:ObjectProperty rdf:about="http://www.w3.org/ns/prov#qualifiedAssociation">
        <rdf:type rdf:resource="&owl;InverseFunctionalProperty"/>
        <rdfs:comment xml:lang="en">If this Activity prov:wasAssociatedWith Agent :ag, then it can qualify the Association using prov:qualifiedAssociation [ a prov:Association;  prov:agent :ag; :foo :bar ].</rdfs:comment>
        <component>agents-responsibility</component>
        <inverse>qualifiedAssociationOf</inverse>
        <category>qualified</category>
        <rdfs:domain rdf:resource="http://www.w3.org/ns/prov#Activity"/>
        <sharesDefinitionWith rdf:resource="http://www.w3.org/ns/prov#Association"/>
        <rdfs:range rdf:resource="http://www.w3.org/ns/prov#Association"/>
        <unqualifiedForm rdf:resource="http://www.w3.org/ns/prov#wasAssociatedWith"/>
    </owl:ObjectProperty>
    


    <!-- http://www.w3.org/ns/prov#qualifiedAttribution -->

    <owl:ObjectProperty rdf:about="http://www.w3.org/ns/prov#qualifiedAttribution">
        <rdf:type rdf:resource="&owl;InverseFunctionalProperty"/>
        <category>qualified</category>
        <component>agents-responsibility</component>
        <inverse>qualifiedAttributionOf</inverse>
        <rdfs:comment xml:lang="en">If this Entity prov:wasAttributedTo Agent :ag, then it can qualify how it was  using prov:qualifiedAttribution [ a prov:Attribution;  prov:agent :ag; :foo :bar ].</rdfs:comment>
        <sharesDefinitionWith rdf:resource="http://www.w3.org/ns/prov#Attribution"/>
        <rdfs:range rdf:resource="http://www.w3.org/ns/prov#Attribution"/>
        <rdfs:domain rdf:resource="http://www.w3.org/ns/prov#Entity"/>
        <unqualifiedForm rdf:resource="http://www.w3.org/ns/prov#wasAttributedTo"/>
    </owl:ObjectProperty>
    


    <!-- http://www.w3.org/ns/prov#qualifiedCommunication -->

    <owl:ObjectProperty rdf:about="http://www.w3.org/ns/prov#qualifiedCommunication">
        <rdf:type rdf:resource="&owl;InverseFunctionalProperty"/>
        <component>entities-activities</component>
        <rdfs:comment xml:lang="en">If this Activity prov:wasInformedBy Activity :a, then it can qualify how it was Inform[ed] using prov:qualifiedCommunication [ a prov:Communication;  prov:activity :a; :foo :bar ].</rdfs:comment>
        <inverse>qualifiedCommunicationOf</inverse>
        <category>qualified</category>
        <rdfs:domain rdf:resource="http://www.w3.org/ns/prov#Activity"/>
        <rdfs:range rdf:resource="http://www.w3.org/ns/prov#Communication"/>
        <sharesDefinitionWith rdf:resource="http://www.w3.org/ns/prov#Communication"/>
        <qualifiedForm rdf:resource="http://www.w3.org/ns/prov#Communication"/>
    </owl:ObjectProperty>
    


    <!-- http://www.w3.org/ns/prov#qualifiedDelegation -->

    <owl:ObjectProperty rdf:about="http://www.w3.org/ns/prov#qualifiedDelegation">
        <rdf:type rdf:resource="&owl;InverseFunctionalProperty"/>
        <category>qualified</category>
        <inverse>qualifiedDelegationOf</inverse>
        <rdfs:comment xml:lang="en">If this Agent prov:actedOnBehalfOf Agent :ag, then it can qualify how with prov:qualifiedResponsibility [ a prov:Responsibility;  prov:agent :ag; :foo :bar ].</rdfs:comment>
        <component>agents-responsibility</component>
        <rdfs:domain rdf:resource="http://www.w3.org/ns/prov#Agent"/>
        <sharesDefinitionWith rdf:resource="http://www.w3.org/ns/prov#Delegation"/>
        <rdfs:range rdf:resource="http://www.w3.org/ns/prov#Delegation"/>
        <unqualifiedForm rdf:resource="http://www.w3.org/ns/prov#actedOnBehalfOf"/>
    </owl:ObjectProperty>
    


    <!-- http://www.w3.org/ns/prov#qualifiedDerivation -->

    <owl:ObjectProperty rdf:about="http://www.w3.org/ns/prov#qualifiedDerivation">
        <rdf:type rdf:resource="&owl;InverseFunctionalProperty"/>
        <rdfs:comment xml:lang="en">If this Entity prov:wasDerivedFrom Entity :e, then it can qualify how it was derived using prov:qualifiedDerivation [ a prov:Derivation;  prov:entity :e; :foo :bar ].</rdfs:comment>
        <inverse>qualifiedDerivationOf</inverse>
        <component>derivations</component>
        <category>qualified</category>
        <sharesDefinitionWith rdf:resource="http://www.w3.org/ns/prov#Derivation"/>
        <rdfs:range rdf:resource="http://www.w3.org/ns/prov#Derivation"/>
        <rdfs:domain rdf:resource="http://www.w3.org/ns/prov#Entity"/>
        <unqualifiedForm rdf:resource="http://www.w3.org/ns/prov#wasDerivedFrom"/>
    </owl:ObjectProperty>
    


    <!-- http://www.w3.org/ns/prov#qualifiedEnd -->

    <owl:ObjectProperty rdf:about="http://www.w3.org/ns/prov#qualifiedEnd">
        <rdf:type rdf:resource="&owl;InverseFunctionalProperty"/>
        <category>qualified</category>
        <inverse>qualifiedEndOf</inverse>
        <component>entities-activities</component>
        <rdfs:comment xml:lang="en">If this Activity prov:wasEndedBy Entity :e1, then it can qualify how it was ended using prov:qualifiedEnd [ a prov:End;  prov:entity :e1; :foo :bar ].</rdfs:comment>
        <rdfs:domain rdf:resource="http://www.w3.org/ns/prov#Activity"/>
        <sharesDefinitionWith rdf:resource="http://www.w3.org/ns/prov#End"/>
        <rdfs:range rdf:resource="http://www.w3.org/ns/prov#End"/>
        <unqualifiedForm rdf:resource="http://www.w3.org/ns/prov#wasEndedBy"/>
    </owl:ObjectProperty>
    


    <!-- http://www.w3.org/ns/prov#qualifiedGeneration -->

    <owl:ObjectProperty rdf:about="http://www.w3.org/ns/prov#qualifiedGeneration">
        <rdf:type rdf:resource="&owl;InverseFunctionalProperty"/>
        <rdfs:comment xml:lang="en">If this Activity prov:generated Entity :e, then it can qualify how it did performed the Generation using prov:qualifiedGeneration [ a prov:Generation;  prov:entity :e; :foo :bar ].</rdfs:comment>
        <inverse>qualifiedGenerationOf</inverse>
        <component>entities-activities</component>
        <category>qualified</category>
        <rdfs:domain rdf:resource="http://www.w3.org/ns/prov#Entity"/>
        <rdfs:range rdf:resource="http://www.w3.org/ns/prov#Generation"/>
        <sharesDefinitionWith rdf:resource="http://www.w3.org/ns/prov#Generation"/>
        <unqualifiedForm rdf:resource="http://www.w3.org/ns/prov#wasGeneratedBy"/>
    </owl:ObjectProperty>
    


    <!-- http://www.w3.org/ns/prov#qualifiedInsertion -->

    <owl:ObjectProperty rdf:about="http://www.w3.org/ns/prov#qualifiedInsertion">
        <component>collections</component>
        <rdfs:comment xml:lang="en">If this Dictionary prov:derivedByInsertionFrom another Dictionary :e, then it can qualify how it did perform the Insertion using prov:qualifiedInsertion [ a prov:Insertion;  prov:dictionary :e; prov:inserted [a prov:KeyValuePair; prov:pairKey &quot;k1&quot;^^xsd:string; prov:pairValue :foo] ].</rdfs:comment>
        <inverse>qualifiedInsertionOf</inverse>
        <category>collections</category>
        <rdfs:domain rdf:resource="http://www.w3.org/ns/prov#Dictionary"/>
        <sharesDefinitionWith rdf:resource="http://www.w3.org/ns/prov#Insertion"/>
        <rdfs:range rdf:resource="http://www.w3.org/ns/prov#Insertion"/>
        <unqualifiedForm rdf:resource="http://www.w3.org/ns/prov#derivedByInsertionFrom"/>
    </owl:ObjectProperty>
    


    <!-- http://www.w3.org/ns/prov#qualifiedInvalidation -->

    <owl:ObjectProperty rdf:about="http://www.w3.org/ns/prov#qualifiedInvalidation">
        <rdf:type rdf:resource="&owl;InverseFunctionalProperty"/>
        <rdfs:comment xml:lang="en">If this Entity prov:wasInvalidatedBy Activity :a, then it can qualify how it was invalidated using prov:qualifiedInvalidation [ a prov:Invalidation;  prov:activity :a; :foo :bar ].</rdfs:comment>
        <component>entities-activities</component>
        <category>qualified</category>
        <inverse>qualifiedInvalidationOf</inverse>
        <rdfs:domain rdf:resource="http://www.w3.org/ns/prov#Entity"/>
        <sharesDefinitionWith rdf:resource="http://www.w3.org/ns/prov#Invalidation"/>
        <rdfs:range rdf:resource="http://www.w3.org/ns/prov#Invalidation"/>
        <unqualifiedForm rdf:resource="http://www.w3.org/ns/prov#wasInvalidatedBy"/>
    </owl:ObjectProperty>
    


    <!-- http://www.w3.org/ns/prov#qualifiedMembership -->

    <owl:ObjectProperty rdf:about="http://www.w3.org/ns/prov#qualifiedMembership">
        <rdfs:label xml:lang="en">qualifiedMembership</rdfs:label>
        <category>collections</category>
        <editorialNote xml:lang="en">This property is NOT inverse functional, since the membership of many distinct KeyValuePairs can be qualified using a single instance of prov:Membership.</editorialNote>
        <component>collections</component>
        <rdfs:comment xml:lang="en">The collection included the specified membership of keys-values.</rdfs:comment>
        <inverse>membershipOf</inverse>
        <rdfs:domain rdf:resource="http://www.w3.org/ns/prov#Dictionary"/>
        <rdfs:range rdf:resource="http://www.w3.org/ns/prov#Membership"/>
        <sharesDefinitionWith rdf:resource="http://www.w3.org/ns/prov#Membership"/>
    </owl:ObjectProperty>
    


    <!-- http://www.w3.org/ns/prov#qualifiedQuotation -->

    <owl:ObjectProperty rdf:about="http://www.w3.org/ns/prov#qualifiedQuotation">
        <rdf:type rdf:resource="&owl;InverseFunctionalProperty"/>
        <category>qualified</category>
        <inverse>qualifiedQuotationOf</inverse>
        <rdfs:comment xml:lang="en">If this Entity prov:wasQuotedFrom Entity :e, then it can qualify how using prov:qualifiedQuotation [ a prov:Quotation;  prov:entity :e; :foo :bar ].</rdfs:comment>
        <component>derivations</component>
        <rdfs:domain rdf:resource="http://www.w3.org/ns/prov#Entity"/>
        <sharesDefinitionWith rdf:resource="http://www.w3.org/ns/prov#Quotation"/>
        <rdfs:range rdf:resource="http://www.w3.org/ns/prov#Quotation"/>
        <unqualifiedForm rdf:resource="http://www.w3.org/ns/prov#wasQuotedFrom"/>
    </owl:ObjectProperty>
    


    <!-- http://www.w3.org/ns/prov#qualifiedRemoval -->

    <owl:ObjectProperty rdf:about="http://www.w3.org/ns/prov#qualifiedRemoval">
        <inverse>removedFromDictionary</inverse>
        <category>collections</category>
        <component>collections</component>
        <rdfs:comment xml:lang="en">If this Dictionary prov:derivedByRemovalFrom another Dictionary :e, then it can qualify how it did perform the Removal using prov:qualifiedRemoval [ a prov:Removal;  prov:dictionary :c; prov:removed &quot;k1&quot;^^xsd:string ].</rdfs:comment>
        <rdfs:domain rdf:resource="http://www.w3.org/ns/prov#Dictionary"/>
        <sharesDefinitionWith rdf:resource="http://www.w3.org/ns/prov#Removal"/>
        <rdfs:range rdf:resource="http://www.w3.org/ns/prov#Removal"/>
        <unqualifiedForm rdf:resource="http://www.w3.org/ns/prov#derivedByRemovalFrom"/>
    </owl:ObjectProperty>
    


    <!-- http://www.w3.org/ns/prov#qualifiedRevision -->

    <owl:ObjectProperty rdf:about="http://www.w3.org/ns/prov#qualifiedRevision">
        <rdf:type rdf:resource="&owl;InverseFunctionalProperty"/>
        <rdfs:comment xml:lang="en">If this Entity prov:wasRevisionOf Entity :e, then it can qualify how it was  revised using prov:qualifiedRevision [ a prov:Revision;  prov:entity :e; :foo :bar ].</rdfs:comment>
        <category>qualified</category>
        <inverse>revisedEntity</inverse>
        <component>derivations</component>
        <rdfs:domain rdf:resource="http://www.w3.org/ns/prov#Entity"/>
        <rdfs:range rdf:resource="http://www.w3.org/ns/prov#Revision"/>
        <sharesDefinitionWith rdf:resource="http://www.w3.org/ns/prov#Revision"/>
        <unqualifiedForm rdf:resource="http://www.w3.org/ns/prov#wasRevisionOf"/>
    </owl:ObjectProperty>
    


    <!-- http://www.w3.org/ns/prov#qualifiedSource -->

    <owl:ObjectProperty rdf:about="http://www.w3.org/ns/prov#qualifiedSource">
        <rdf:type rdf:resource="&owl;InverseFunctionalProperty"/>
        <component>derivations</component>
        <category>qualified</category>
        <inverse>qualifiedSourceOf</inverse>
        <rdfs:comment xml:lang="en">If this Entity prov:hadOriginalSource Entity :e, then it can qualify how using prov:qualifiedSource [ a prov:Source; prov:entity :e; :foo :bar ].</rdfs:comment>
        <rdfs:domain rdf:resource="http://www.w3.org/ns/prov#Entity"/>
        <rdfs:range rdf:resource="http://www.w3.org/ns/prov#Source"/>
        <sharesDefinitionWith rdf:resource="http://www.w3.org/ns/prov#Source"/>
        <unqualifiedForm rdf:resource="http://www.w3.org/ns/prov#hadPrimarySource"/>
    </owl:ObjectProperty>
    


    <!-- http://www.w3.org/ns/prov#qualifiedStart -->

    <owl:ObjectProperty rdf:about="http://www.w3.org/ns/prov#qualifiedStart">
        <rdf:type rdf:resource="&owl;InverseFunctionalProperty"/>
        <inverse>qualifiedStartOf</inverse>
        <category>qualified</category>
        <component>entities-activities</component>
        <rdfs:comment xml:lang="en">If this Activity prov:wasStartedBy Entity :e1, then it can qualify how it was started using prov:qualifiedStart [ a prov:Start;  prov:entity :e1; :foo :bar ].</rdfs:comment>
        <rdfs:domain rdf:resource="http://www.w3.org/ns/prov#Activity"/>
        <rdfs:range rdf:resource="http://www.w3.org/ns/prov#Start"/>
        <sharesDefinitionWith rdf:resource="http://www.w3.org/ns/prov#Start"/>
        <unqualifiedForm rdf:resource="http://www.w3.org/ns/prov#wasStartedBy"/>
    </owl:ObjectProperty>
    


    <!-- http://www.w3.org/ns/prov#qualifiedTrace -->

    <owl:ObjectProperty rdf:about="http://www.w3.org/ns/prov#qualifiedTrace">
        <rdf:type rdf:resource="&owl;InverseFunctionalProperty"/>
        <inverse>qualifiedTraceOf</inverse>
        <category>qualified</category>
        <rdfs:comment xml:lang="en">If this prov:wasAttributedTo Entity :e, then it can qualify how using prov:qualifiedTrace [ a prov:Trace;  prov:entity :e; :foo :bar ]. If this prov:wasAttributedTo Activity :a, then it can qualify how using prov:qualifiedTrace [ a prov:Trace;  prov:activity :a; :foo :bar ].</rdfs:comment>
        <component>derivations</component>
        <rdfs:domain rdf:resource="http://www.w3.org/ns/prov#Entity"/>
        <rdfs:range rdf:resource="http://www.w3.org/ns/prov#Trace"/>
        <sharesDefinitionWith rdf:resource="http://www.w3.org/ns/prov#Trace"/>
        <unqualifiedForm rdf:resource="http://www.w3.org/ns/prov#tracedTo"/>
    </owl:ObjectProperty>
    


    <!-- http://www.w3.org/ns/prov#qualifiedUsage -->

    <owl:ObjectProperty rdf:about="http://www.w3.org/ns/prov#qualifiedUsage">
        <rdf:type rdf:resource="&owl;InverseFunctionalProperty"/>
        <category>qualified</category>
        <inverse>qualifiedUsingActivity</inverse>
        <component>entities-activities</component>
        <rdfs:comment xml:lang="en">If this Activity prov:used Entity :e, then it can qualify how it used it using prov:qualifiedUsage [ a prov:Usage; prov:entity :e; :foo :bar ].</rdfs:comment>
        <rdfs:domain rdf:resource="http://www.w3.org/ns/prov#Activity"/>
        <sharesDefinitionWith rdf:resource="http://www.w3.org/ns/prov#Usage"/>
        <rdfs:range rdf:resource="http://www.w3.org/ns/prov#Usage"/>
        <unqualifiedForm rdf:resource="http://www.w3.org/ns/prov#used"/>
    </owl:ObjectProperty>
    


    <!-- http://www.w3.org/ns/prov#specializationOf -->

    <owl:ObjectProperty rdf:about="http://www.w3.org/ns/prov#specializationOf">
        <rdf:type rdf:resource="&owl;AsymmetricProperty"/>
        <rdf:type rdf:resource="&owl;IrreflexiveProperty"/>
        <rdf:type rdf:resource="&owl;TransitiveProperty"/>
        <component>alternate</component>
        <category>expanded</category>
        <prov-dm>http://dvcs.w3.org/hg/prov/raw-file/default/model/prov-dm.html#term-specialization</prov-dm>
        <definition>An entity is a specialization of another if they both refer to some common thing but the former is a more constrained entity than the former. The common entity does not need to be identified.</definition>
        <inverse>generalizationOf</inverse>
        <prov-n>http://dvcs.w3.org/hg/prov/raw-file/default/model/prov-n.html#expression-specialization</prov-n>
        <rdfs:comment xml:lang="en">An entity is a specialization of another if they both refer to some common thing but the former is a more constrained entity than the former. The common entity does not need to be identified.</rdfs:comment>
        <prov-dm-constraints>http://dvcs.w3.org/hg/prov/raw-file/default/model/prov-dm-constraints.html#term-Specialization</prov-dm-constraints>
        <rdfs:range rdf:resource="http://www.w3.org/ns/prov#Entity"/>
        <rdfs:domain rdf:resource="http://www.w3.org/ns/prov#Entity"/>
        <rdfs:seeAlso rdf:resource="http://www.w3.org/ns/prov#alternateOf"/>
        <rdfs:subPropertyOf rdf:resource="http://www.w3.org/ns/prov#alternateOf"/>
    </owl:ObjectProperty>
    


    <!-- http://www.w3.org/ns/prov#tracedTo -->

    <owl:ObjectProperty rdf:about="http://www.w3.org/ns/prov#tracedTo">
        <rdf:type rdf:resource="&owl;TransitiveProperty"/>
        <component>derivations</component>
        <category>expanded</category>
        <rdfs:comment xml:lang="en">An object property to link back an entity to another by means of derivation or responsibility relations, possibly repeatedly traversed.</rdfs:comment>
        <inverse>tracedFrom</inverse>
        <rdfs:range rdf:resource="http://www.w3.org/ns/prov#Entity"/>
        <rdfs:domain rdf:resource="http://www.w3.org/ns/prov#Entity"/>
        <qualifiedForm rdf:resource="http://www.w3.org/ns/prov#Trace"/>
        <rdfs:subPropertyOf rdf:resource="http://www.w3.org/ns/prov#involved"/>
        <qualifiedForm rdf:resource="http://www.w3.org/ns/prov#qualifiedTrace"/>
        <owl:propertyChainAxiom rdf:parseType="Collection">
            <rdf:Description rdf:about="http://www.w3.org/ns/prov#qualifiedTrace"/>
            <rdf:Description rdf:about="http://www.w3.org/ns/prov#entity"/>
        </owl:propertyChainAxiom>
    </owl:ObjectProperty>
    


    <!-- http://www.w3.org/ns/prov#used -->

    <owl:ObjectProperty rdf:about="http://www.w3.org/ns/prov#used">
        <rdf:type rdf:resource="&owl;AsymmetricProperty"/>
        <rdf:type rdf:resource="&owl;IrreflexiveProperty"/>
        <inverse>wasUsedBy</inverse>
        <rdfs:comment xml:lang="en">A prov:Entity that was used by this prov:Activity. For example, :baking prov:used :spoon, :egg, :oven .</rdfs:comment>
        <category>starting-point</category>
        <component>entities-activities</component>
        <rdfs:domain rdf:resource="http://www.w3.org/ns/prov#Activity"/>
        <rdfs:range rdf:resource="http://www.w3.org/ns/prov#Entity"/>
        <qualifiedForm rdf:resource="http://www.w3.org/ns/prov#Usage"/>
        <rdfs:subPropertyOf rdf:resource="http://www.w3.org/ns/prov#involved"/>
        <qualifiedForm rdf:resource="http://www.w3.org/ns/prov#qualifiedUsage"/>
        <owl:propertyChainAxiom rdf:parseType="Collection">
            <rdf:Description rdf:about="http://www.w3.org/ns/prov#qualifiedUsage"/>
            <rdf:Description rdf:about="http://www.w3.org/ns/prov#entity"/>
        </owl:propertyChainAxiom>
    </owl:ObjectProperty>
    


    <!-- http://www.w3.org/ns/prov#wasAssociatedWith -->

    <owl:ObjectProperty rdf:about="http://www.w3.org/ns/prov#wasAssociatedWith">
        <component>agents-responsibility</component>
        <inverse>wasAssociateFor</inverse>
        <rdfs:comment xml:lang="en">An prov:Agent that had some (unspecified) responsibility for the occurrence of this prov:Activity.</rdfs:comment>
        <category>starting-point</category>
        <rdfs:domain rdf:resource="http://www.w3.org/ns/prov#Activity"/>
        <rdfs:range rdf:resource="http://www.w3.org/ns/prov#Agent"/>
        <qualifiedForm rdf:resource="http://www.w3.org/ns/prov#Association"/>
        <rdfs:subPropertyOf rdf:resource="http://www.w3.org/ns/prov#involved"/>
        <qualifiedForm rdf:resource="http://www.w3.org/ns/prov#qualifiedAssociation"/>
        <owl:propertyChainAxiom rdf:parseType="Collection">
            <rdf:Description rdf:about="http://www.w3.org/ns/prov#qualifiedAssociation"/>
            <rdf:Description rdf:about="http://www.w3.org/ns/prov#agent"/>
        </owl:propertyChainAxiom>
    </owl:ObjectProperty>
    


    <!-- http://www.w3.org/ns/prov#wasAttributedTo -->

    <owl:ObjectProperty rdf:about="http://www.w3.org/ns/prov#wasAttributedTo">
        <definition>Attribution is the ascribing of an entity to an agent.</definition>
        <rdfs:comment xml:lang="en">Attribution is the ascribing of an entity to an agent.</rdfs:comment>
        <component>agents-responsibility</component>
        <category>starting-point</category>
        <inverse>contributed</inverse>
        <rdfs:range rdf:resource="http://www.w3.org/ns/prov#Agent"/>
        <qualifiedForm rdf:resource="http://www.w3.org/ns/prov#Attribution"/>
        <rdfs:domain rdf:resource="http://www.w3.org/ns/prov#Entity"/>
        <qualifiedForm rdf:resource="http://www.w3.org/ns/prov#qualifiedAttribution"/>
        <rdfs:subPropertyOf rdf:resource="http://www.w3.org/ns/prov#tracedTo"/>
        <owl:propertyChainAxiom rdf:parseType="Collection">
            <rdf:Description rdf:about="http://www.w3.org/ns/prov#qualifiedAttribution"/>
            <rdf:Description rdf:about="http://www.w3.org/ns/prov#agent"/>
        </owl:propertyChainAxiom>
    </owl:ObjectProperty>
    <owl:Axiom>
        <prov-dm-constraints>http://dvcs.w3.org/hg/prov/raw-file/default/model/prov-constraints.html#traceability-inference</prov-dm-constraints>
        <rdfs:comment>Attribution is a particular case of trace (see http://www.w3.org/TR/prov-dm/#concept-trace), in the sense that it links an entity to the agent that ascribed it.</rdfs:comment>
        <definition>IF wasAttributedTo(e2,ag1,aAttr) holds, THEN tracedTo(e2,ag1) also holds. </definition>
        <owl:annotatedProperty rdf:resource="&rdfs;subPropertyOf"/>
        <owl:annotatedTarget rdf:resource="http://www.w3.org/ns/prov#tracedTo"/>
        <owl:annotatedSource rdf:resource="http://www.w3.org/ns/prov#wasAttributedTo"/>
    </owl:Axiom>
    


    <!-- http://www.w3.org/ns/prov#wasDerivedFrom -->

    <owl:ObjectProperty rdf:about="http://www.w3.org/ns/prov#wasDerivedFrom">
        <rdf:type rdf:resource="&owl;AsymmetricProperty"/>
        <rdf:type rdf:resource="&owl;IrreflexiveProperty"/>
        <inverse>hadDerivation</inverse>
        <definition xml:lang="en">A derivation is a transformation of an entity into another, a construction of an entity into another, or an update of an entity, resulting in a new one.</definition>
        <rdfs:comment xml:lang="en">A derivation is a transformation of an entity into another, a construction of an entity into another, or an update of an entity, resulting in a new one.</rdfs:comment>
        <category>starting-point</category>
        <component>derivations</component>
        <rdfs:isDefinedBy rdf:resource="http://www.w3.org/ns/prov#"/>
        <qualifiedForm rdf:resource="http://www.w3.org/ns/prov#Derivation"/>
        <rdfs:range rdf:resource="http://www.w3.org/ns/prov#Entity"/>
        <rdfs:domain rdf:resource="http://www.w3.org/ns/prov#Entity"/>
        <qualifiedForm rdf:resource="http://www.w3.org/ns/prov#qualifiedDerivation"/>
        <rdfs:subPropertyOf rdf:resource="http://www.w3.org/ns/prov#tracedTo"/>
        <owl:propertyChainAxiom rdf:parseType="Collection">
            <rdf:Description rdf:about="http://www.w3.org/ns/prov#qualifiedDerivation"/>
            <rdf:Description rdf:about="http://www.w3.org/ns/prov#entity"/>
        </owl:propertyChainAxiom>
    </owl:ObjectProperty>
    <owl:Axiom>
        <rdfs:comment>Derivation is a particular case of trace (see http://www.w3.org/TR/prov-dm/#term-trace), since it links an entity to another entity that contributed to its existence.</rdfs:comment>
        <owl:annotatedProperty rdf:resource="&rdfs;subPropertyOf"/>
        <owl:annotatedTarget rdf:resource="http://www.w3.org/ns/prov#tracedTo"/>
        <owl:annotatedSource rdf:resource="http://www.w3.org/ns/prov#wasDerivedFrom"/>
    </owl:Axiom>
    


    <!-- http://www.w3.org/ns/prov#wasEndedBy -->

    <owl:ObjectProperty rdf:about="http://www.w3.org/ns/prov#wasEndedBy">
        <category>expanded</category>
        <component>entities-activities</component>
        <rdfs:comment xml:lang="en">End is when an activity is deemed to have ended. An end may refer to an entity, known as trigger, that terminated the activity.</rdfs:comment>
        <inverse>ended</inverse>
        <editorialNote xml:lang="en">was{Started,Ended}By do not have anything to do with agent/attribution. -Luc 20 April 2012</editorialNote>
        <rdfs:domain rdf:resource="http://www.w3.org/ns/prov#Activity"/>
        <qualifiedForm rdf:resource="http://www.w3.org/ns/prov#End"/>
        <rdfs:range rdf:resource="http://www.w3.org/ns/prov#Entity"/>
        <rdfs:subPropertyOf rdf:resource="http://www.w3.org/ns/prov#involved"/>
        <qualifiedForm rdf:resource="http://www.w3.org/ns/prov#qualifiedEnd"/>
        <owl:propertyChainAxiom rdf:parseType="Collection">
            <rdf:Description rdf:about="http://www.w3.org/ns/prov#qualifiedEnd"/>
            <rdf:Description rdf:about="http://www.w3.org/ns/prov#entity"/>
        </owl:propertyChainAxiom>
    </owl:ObjectProperty>
    


    <!-- http://www.w3.org/ns/prov#wasGeneratedBy -->

    <owl:ObjectProperty rdf:about="http://www.w3.org/ns/prov#wasGeneratedBy">
        <rdf:type rdf:resource="&owl;AsymmetricProperty"/>
        <rdf:type rdf:resource="&owl;FunctionalProperty"/>
        <rdf:type rdf:resource="&owl;IrreflexiveProperty"/>
        <inverse>generated</inverse>
        <category>starting-point</category>
        <component>entities-activities</component>
        <rdfs:comment xml:lang="en">wasGeneratedBy links Entitites with Activity representing that entity was generated as a result of Activity</rdfs:comment>
        <rdfs:range rdf:resource="http://www.w3.org/ns/prov#Activity"/>
        <rdfs:domain rdf:resource="http://www.w3.org/ns/prov#Entity"/>
        <qualifiedForm rdf:resource="http://www.w3.org/ns/prov#Generation"/>
        <rdfs:subPropertyOf rdf:resource="http://www.w3.org/ns/prov#involved"/>
        <qualifiedForm rdf:resource="http://www.w3.org/ns/prov#qualifiedGeneration"/>
        <owl:propertyChainAxiom rdf:parseType="Collection">
            <rdf:Description rdf:about="http://www.w3.org/ns/prov#qualifiedGeneration"/>
            <rdf:Description rdf:about="http://www.w3.org/ns/prov#activity"/>
        </owl:propertyChainAxiom>
    </owl:ObjectProperty>
    


    <!-- http://www.w3.org/ns/prov#wasInformedBy -->

    <owl:ObjectProperty rdf:about="http://www.w3.org/ns/prov#wasInformedBy">
        <inverse>informed</inverse>
        <rdfs:comment xml:lang="en">An activity a2 is dependent on or informed by another activity a1, by way of some unspecified entity that is generated by a1 and used by a2.</rdfs:comment>
        <category>starting-point</category>
        <component>entities-activities</component>
        <rdfs:domain rdf:resource="http://www.w3.org/ns/prov#Activity"/>
        <rdfs:range rdf:resource="http://www.w3.org/ns/prov#Activity"/>
        <qualifiedForm rdf:resource="http://www.w3.org/ns/prov#Communication"/>
        <rdfs:subPropertyOf rdf:resource="http://www.w3.org/ns/prov#involved"/>
        <qualifiedForm rdf:resource="http://www.w3.org/ns/prov#qualifiedCommunication"/>
        <owl:propertyChainAxiom rdf:parseType="Collection">
            <rdf:Description rdf:about="http://www.w3.org/ns/prov#qualifiedCommunication"/>
            <rdf:Description rdf:about="http://www.w3.org/ns/prov#entity"/>
        </owl:propertyChainAxiom>
    </owl:ObjectProperty>
    


    <!-- http://www.w3.org/ns/prov#wasInvalidatedBy -->

    <owl:ObjectProperty rdf:about="http://www.w3.org/ns/prov#wasInvalidatedBy">
        <inverse>invalidated</inverse>
        <category>expanded</category>
        <component>entities-activities</component>
        <rdfs:range rdf:resource="http://www.w3.org/ns/prov#Activity"/>
        <rdfs:domain rdf:resource="http://www.w3.org/ns/prov#Entity"/>
        <qualifiedForm rdf:resource="http://www.w3.org/ns/prov#Invalidation"/>
        <rdfs:subPropertyOf rdf:resource="http://www.w3.org/ns/prov#involved"/>
        <qualifiedForm rdf:resource="http://www.w3.org/ns/prov#qualifiedInvalidation"/>
        <owl:propertyChainAxiom rdf:parseType="Collection">
            <rdf:Description rdf:about="http://www.w3.org/ns/prov#qualifiedInvalidation"/>
            <rdf:Description rdf:about="http://www.w3.org/ns/prov#activity"/>
        </owl:propertyChainAxiom>
    </owl:ObjectProperty>
    


    <!-- http://www.w3.org/ns/prov#wasQuotedFrom -->

    <owl:ObjectProperty rdf:about="http://www.w3.org/ns/prov#wasQuotedFrom">
        <category>expanded</category>
        <component>derivations</component>
        <rdfs:comment xml:lang="en">An entity is derived from an original entity by copying, or &quot;quoting&quot;, some or all of it.</rdfs:comment>
        <inverse>quotedAs</inverse>
        <rdfs:domain rdf:resource="http://www.w3.org/ns/prov#Entity"/>
        <rdfs:range rdf:resource="http://www.w3.org/ns/prov#Entity"/>
        <qualifiedForm rdf:resource="http://www.w3.org/ns/prov#Quotation"/>
        <qualifiedForm rdf:resource="http://www.w3.org/ns/prov#qualifiedQuotation"/>
        <rdfs:subPropertyOf rdf:resource="http://www.w3.org/ns/prov#wasDerivedFrom"/>
        <owl:propertyChainAxiom rdf:parseType="Collection">
            <rdf:Description rdf:about="http://www.w3.org/ns/prov#qualifiedQuotation"/>
            <rdf:Description rdf:about="http://www.w3.org/ns/prov#entity"/>
        </owl:propertyChainAxiom>
    </owl:ObjectProperty>
    <owl:Axiom>
        <rdfs:comment>Quotation is a particular case of derivation (see http://www.w3.org/TR/prov-dm/#term-quotation) in which an entity is derived from an original entity by copying, or &quot;quoting&quot;, some or all of it. </rdfs:comment>
        <owl:annotatedProperty rdf:resource="&rdfs;subPropertyOf"/>
        <owl:annotatedTarget rdf:resource="http://www.w3.org/ns/prov#wasDerivedFrom"/>
        <owl:annotatedSource rdf:resource="http://www.w3.org/ns/prov#wasQuotedFrom"/>
    </owl:Axiom>
    


    <!-- http://www.w3.org/ns/prov#wasRevisionOf -->

    <owl:ObjectProperty rdf:about="http://www.w3.org/ns/prov#wasRevisionOf">
        <component>derivations</component>
        <rdfs:comment xml:lang="en">A revision is a derivation that revises an entity into a revised version.</rdfs:comment>
        <inverse>hadRevision</inverse>
        <category>expanded</category>
        <rdfs:range rdf:resource="http://www.w3.org/ns/prov#Entity"/>
        <rdfs:domain rdf:resource="http://www.w3.org/ns/prov#Entity"/>
        <qualifiedForm rdf:resource="http://www.w3.org/ns/prov#Revision"/>
        <qualifiedForm rdf:resource="http://www.w3.org/ns/prov#qualifiedRevision"/>
        <rdfs:subPropertyOf rdf:resource="http://www.w3.org/ns/prov#wasDerivedFrom"/>
        <owl:propertyChainAxiom rdf:parseType="Collection">
            <rdf:Description rdf:about="http://www.w3.org/ns/prov#qualifiedRevision"/>
            <rdf:Description rdf:about="http://www.w3.org/ns/prov#entity"/>
        </owl:propertyChainAxiom>
    </owl:ObjectProperty>
    <owl:Axiom>
        <rdfs:comment>Revision is a derivation (see http://www.w3.org/TR/prov-dm/#term-Revision). Moreover, according to 
http://dvcs.w3.org/hg/prov/raw-file/default/model/prov-dm-constraints.html#term-Revision 23 April 2012 &#39;wasRevisionOf is a strict sub-relation of wasDerivedFrom since two entities e2 and e1 may satisfy wasDerivedFrom(e2,e1) without being a variant of each other.&#39;</rdfs:comment>
        <owl:annotatedProperty rdf:resource="&rdfs;subPropertyOf"/>
        <owl:annotatedTarget rdf:resource="http://www.w3.org/ns/prov#wasDerivedFrom"/>
        <owl:annotatedSource rdf:resource="http://www.w3.org/ns/prov#wasRevisionOf"/>
    </owl:Axiom>
    


    <!-- http://www.w3.org/ns/prov#wasStartedBy -->

    <owl:ObjectProperty rdf:about="http://www.w3.org/ns/prov#wasStartedBy">
        <inverse>started</inverse>
        <category>expanded</category>
        <component>entities-activities</component>
        <rdfs:comment xml:lang="en">Start is when an activity is deemed to have started. A start may refer to an entity, known as trigger, that initiated the activity.</rdfs:comment>
        <editorialNote xml:lang="en">was{Started,Ended}By do not have anything to do with agent/attribution. -Luc 20 April 2012</editorialNote>
        <rdfs:domain rdf:resource="http://www.w3.org/ns/prov#Activity"/>
        <rdfs:range rdf:resource="http://www.w3.org/ns/prov#Entity"/>
        <qualifiedForm rdf:resource="http://www.w3.org/ns/prov#Start"/>
        <rdfs:subPropertyOf rdf:resource="http://www.w3.org/ns/prov#involved"/>
        <qualifiedForm rdf:resource="http://www.w3.org/ns/prov#qualifiedStart"/>
        <owl:propertyChainAxiom rdf:parseType="Collection">
            <rdf:Description rdf:about="http://www.w3.org/ns/prov#qualifiedStart"/>
            <rdf:Description rdf:about="http://www.w3.org/ns/prov#entity"/>
        </owl:propertyChainAxiom>
    </owl:ObjectProperty>
    


    <!-- 
    ///////////////////////////////////////////////////////////////////////////////////////
    //
    // Data properties
    //
    ///////////////////////////////////////////////////////////////////////////////////////
     -->

    


    <!-- http://www.w3.org/ns/prov#atTime -->

    <owl:DatatypeProperty rdf:about="http://www.w3.org/ns/prov#atTime">
        <rdf:type rdf:resource="&owl;FunctionalProperty"/>
        <component>entities-activities</component>
        <category>qualified</category>
        <rdfs:comment>The time at which an InstantaneousEvent occurred, in the form of xsd:dateTime. This property is predominantly used on Involvements such as Generation, Usage, and Invalidation.</rdfs:comment>
        <rdfs:range rdf:resource="&xsd;dateTime"/>
        <sharesDefinitionWith rdf:resource="http://www.w3.org/ns/prov#InstantaneousEvent"/>
        <rdfs:domain rdf:resource="http://www.w3.org/ns/prov#InstantaneousEvent"/>
        <unqualifiedForm rdf:resource="http://www.w3.org/ns/prov#endedAtTime"/>
        <unqualifiedForm rdf:resource="http://www.w3.org/ns/prov#generatedAtTime"/>
        <unqualifiedForm rdf:resource="http://www.w3.org/ns/prov#invalidatedAtTime"/>
        <unqualifiedForm rdf:resource="http://www.w3.org/ns/prov#startedAtTime"/>
    </owl:DatatypeProperty>
    


    <!-- http://www.w3.org/ns/prov#endedAtTime -->

    <owl:DatatypeProperty rdf:about="http://www.w3.org/ns/prov#endedAtTime">
        <rdf:type rdf:resource="&owl;FunctionalProperty"/>
        <rdfs:comment xml:lang="en">The time at which an activity ended. See also prov:startedAtTime.</rdfs:comment>
        <component>entities-activities</component>
        <category>starting-point</category>
        <rdfs:range rdf:resource="&xsd;dateTime"/>
        <rdfs:domain rdf:resource="http://www.w3.org/ns/prov#Activity"/>
        <qualifiedForm rdf:resource="http://www.w3.org/ns/prov#End"/>
        <qualifiedForm rdf:resource="http://www.w3.org/ns/prov#atTime"/>
    </owl:DatatypeProperty>
    


    <!-- http://www.w3.org/ns/prov#generatedAtTime -->

    <owl:DatatypeProperty rdf:about="http://www.w3.org/ns/prov#generatedAtTime">
        <rdf:type rdf:resource="&owl;FunctionalProperty"/>
        <category>expanded</category>
        <component>entities-activities</component>
        <rdfs:comment xml:lang="en">The time at which an entity was completely created.</rdfs:comment>
        <rdfs:range rdf:resource="&xsd;dateTime"/>
        <rdfs:domain rdf:resource="http://www.w3.org/ns/prov#Entity"/>
        <qualifiedForm rdf:resource="http://www.w3.org/ns/prov#Generation"/>
        <qualifiedForm rdf:resource="http://www.w3.org/ns/prov#atTime"/>
    </owl:DatatypeProperty>
    


    <!-- http://www.w3.org/ns/prov#invalidatedAtTime -->

    <owl:DatatypeProperty rdf:about="http://www.w3.org/ns/prov#invalidatedAtTime">
        <rdf:type rdf:resource="&owl;FunctionalProperty"/>
        <category>expanded</category>
        <component>entities-activities</component>
        <rdfs:comment xml:lang="en">The time at which an entity began to be invalidated (i.e., no longer usable).</rdfs:comment>
        <rdfs:range rdf:resource="&xsd;dateTime"/>
        <rdfs:domain rdf:resource="http://www.w3.org/ns/prov#Entity"/>
        <qualifiedForm rdf:resource="http://www.w3.org/ns/prov#Invalidation"/>
        <qualifiedForm rdf:resource="http://www.w3.org/ns/prov#atTime"/>
    </owl:DatatypeProperty>
    


    <!-- http://www.w3.org/ns/prov#pairKey -->

    <owl:DatatypeProperty rdf:about="http://www.w3.org/ns/prov#pairKey">
        <rdf:type rdf:resource="&owl;FunctionalProperty"/>
        <definition xml:lang="en">The key with which an Entity has been inserted into a prov:Dictionary; a key is expected to be unique within each prov:Dictionary.</definition>
        <category>collections</category>
        <component>collections</component>
        <rdfs:comment xml:lang="en">The key of a KeyValuePair, which is an element of a prov:Dictionary. See also prov:pairValue.</rdfs:comment>
        <rdfs:range rdf:resource="&rdfs;Literal"/>
        <rdfs:domain rdf:resource="http://www.w3.org/ns/prov#KeyValuePair"/>
    </owl:DatatypeProperty>
    


    <!-- http://www.w3.org/ns/prov#provenanceUriTemplate -->

    <owl:DatatypeProperty rdf:about="http://www.w3.org/ns/prov#provenanceUriTemplate">
        <rdfs:comment xml:lang="en">Relates a provenance service to a URI template string for constructing provenance-URIs.</rdfs:comment>
        <category>access-and-query</category>
        <prov-aq xml:lang="en">http://dvcs.w3.org/hg/prov/raw-file/tip/paq/prov-aq.html#todo</prov-aq>
    </owl:DatatypeProperty>
    


    <!-- http://www.w3.org/ns/prov#removed -->

    <owl:DatatypeProperty rdf:about="http://www.w3.org/ns/prov#removed">
        <rdfs:label xml:lang="en">removed</rdfs:label>
        <component>collections</component>
        <editorialNote xml:lang="en">The value of this property refers to the value of a KeyValuePair&#39;s prov:pairKey property.</editorialNote>
        <prov-dm>http://dvcs.w3.org/hg/prov/raw-file/default/model/prov-dm.html#term-dictionary-removal</prov-dm>
        <editorsDefinition xml:lang="en">The key removed from a prov:Dictionary in a Removal, resulting in a new prov:Dictionary.</editorsDefinition>
        <category>collections</category>
        <rdfs:range rdf:resource="&rdfs;Literal"/>
        <rdfs:domain rdf:resource="http://www.w3.org/ns/prov#Removal"/>
    </owl:DatatypeProperty>
    


    <!-- http://www.w3.org/ns/prov#startedAtTime -->

    <owl:DatatypeProperty rdf:about="http://www.w3.org/ns/prov#startedAtTime">
        <rdf:type rdf:resource="&owl;FunctionalProperty"/>
        <category>starting-point</category>
        <component>entities-activities</component>
        <rdfs:comment xml:lang="en">The time at which an activity started. See also prov:endedAtTime.</rdfs:comment>
        <rdfs:range rdf:resource="&xsd;dateTime"/>
        <rdfs:domain rdf:resource="http://www.w3.org/ns/prov#Activity"/>
        <qualifiedForm rdf:resource="http://www.w3.org/ns/prov#Start"/>
        <qualifiedForm rdf:resource="http://www.w3.org/ns/prov#atTime"/>
    </owl:DatatypeProperty>
    


    <!-- http://www.w3.org/ns/prov#value -->

    <owl:DatatypeProperty rdf:about="http://www.w3.org/ns/prov#value">
        <prov-dm-constraints></prov-dm-constraints>
        <category>expanded</category>
        <editorialNote>The editor&#39;s definition comes from http://www.w3.org/TR/rdf-primer/#rdfvalue</editorialNote>
        <editorialNote>This property serves the same purpose as rdf:value, but has been reintroduced to avoid some of the definitional ambiguity in the RDF specification (specifically, &#39;may be used in describing structured values&#39;).</editorialNote>
        <component>entities-activities</component>
        <rdfs:comment xml:lang="en">Provides a value for an Entity.</rdfs:comment>
        <prov-dm>http://dvcs.w3.org/hg/prov/raw-file/default/model/prov-dm.html#term-attribute-value</prov-dm>
        <prov-n></prov-n>
        <editorsDefinition xml:lang="en">The main value (if there is one) of a structured value.</editorsDefinition>
        <rdfs:domain rdf:resource="http://www.w3.org/ns/prov#Entity"/>
    </owl:DatatypeProperty>
    


    <!-- 
    ///////////////////////////////////////////////////////////////////////////////////////
    //
    // Classes
    //
    ///////////////////////////////////////////////////////////////////////////////////////
     -->

    


    <!-- http://www.w3.org/2002/07/owl#Thing -->

    <owl:Class rdf:about="&owl;Thing"/>
    


    <!-- http://www.w3.org/ns/prov#Activity -->

    <owl:Class rdf:about="http://www.w3.org/ns/prov#Activity">
        <rdfs:label>Activity</rdfs:label>
        <owl:disjointWith rdf:resource="http://www.w3.org/ns/prov#Entity"/>
        <prov-dm rdf:datatype="&xsd;anyURI">http://dvcs.w3.org/hg/prov/raw-file/default/model/prov-dm.html#section-entity-activity</prov-dm>
        <component>entities-activities</component>
        <prov-n>http://dvcs.w3.org/hg/prov/raw-file/default/model/prov-n.html#expression-Activity</prov-n>
        <rdfs:comment xml:lang="en">An activity is something that occurs over a period of time and acts upon or with entities. This action can take multiple forms: consuming, processing, transforming, modifying, relocating, using, generating, or being associated with entities. Activities that operate on digital entities may for example move, copy, or duplicate them.</rdfs:comment>
        <category>starting-point</category>
        <prov-dm-constraints>http://dvcs.w3.org/hg/prov/raw-file/default/model/prov-dm-constraints.html#term-Activity</prov-dm-constraints>
        <definition>An activity is something that occurs over a period of time and acts upon or with entities; it may include consuming, processing, transforming, modifying, relocating, using, or generating entities.</definition>
    </owl:Class>
    


    <!-- http://www.w3.org/ns/prov#ActivityInvolvement -->

    <owl:Class rdf:about="http://www.w3.org/ns/prov#ActivityInvolvement">
        <rdfs:label>ActivityInvolvement</rdfs:label>
        <rdfs:subClassOf rdf:resource="http://www.w3.org/ns/prov#Involvement"/>
        <rdfs:subClassOf>
            <owl:Restriction>
                <owl:onProperty rdf:resource="http://www.w3.org/ns/prov#hadActivity"/>
                <owl:maxCardinality rdf:datatype="&xsd;nonNegativeInteger">0</owl:maxCardinality>
            </owl:Restriction>
        </rdfs:subClassOf>
        <owl:disjointWith rdf:resource="http://www.w3.org/ns/prov#EntityInvolvement"/>
        <category>qualified</category>
        <editorsDefinition xml:lang="en">prov:ActivityInvolvement provides descriptions of any binary involvement between any instance and an prov:Activity. The property prov:activity is used to reference the object of the triple being described.</editorsDefinition>
        <rdfs:seeAlso rdf:resource="http://www.w3.org/ns/prov#activity"/>
    </owl:Class>
    


    <!-- http://www.w3.org/ns/prov#Agent -->

    <owl:Class rdf:about="http://www.w3.org/ns/prov#Agent">
        <rdfs:label>Agent</rdfs:label>
        <owl:disjointWith rdf:resource="http://www.w3.org/ns/prov#InstantaneousEvent"/>
        <prov-dm-constraints>http://dvcs.w3.org/hg/prov/raw-file/default/model/prov-dm-constraints.html#term-Agent</prov-dm-constraints>
        <definition xml:lang="en">An agent is something that bears some form of responsibility for an activity taking place or for the existence of an entity.</definition>
        <prov-n>http://dvcs.w3.org/hg/prov/raw-file/default/model/prov-n.html#expression-Agent</prov-n>
        <category>starting-point</category>
        <rdfs:comment xml:lang="en">An agent is a type of entity that bears some form of responsibility for an activity taking place.</rdfs:comment>
        <component>agents-responsibility</component>
        <prov-dm>http://dvcs.w3.org/hg/prov/raw-file/default/model/prov-dm.html#term-Agent</prov-dm>
    </owl:Class>
    


    <!-- http://www.w3.org/ns/prov#AgentInvolvement -->

    <owl:Class rdf:about="http://www.w3.org/ns/prov#AgentInvolvement">
        <rdfs:label>AgentInvolvement</rdfs:label>
        <rdfs:subClassOf rdf:resource="http://www.w3.org/ns/prov#Involvement"/>
        <editorsDefinition xml:lang="en">prov:AgentInvolvement provides descriptions of any binary involvement between any instance and an prov:Agent. The property prov:agent is used to reference the object of the triple being described.</editorsDefinition>
        <category>qualified</category>
        <rdfs:seeAlso rdf:resource="http://www.w3.org/ns/prov#agent"/>
    </owl:Class>
    


    <!-- http://www.w3.org/ns/prov#Association -->

    <owl:Class rdf:about="http://www.w3.org/ns/prov#Association">
        <rdfs:label>Association</rdfs:label>
        <rdfs:subClassOf rdf:resource="http://www.w3.org/ns/prov#AgentInvolvement"/>
        <prov-n>http://dvcs.w3.org/hg/prov/raw-file/default/model/prov-n.html#expression-Association</prov-n>
        <component>agents-responsibility</component>
        <prov-dm>http://dvcs.w3.org/hg/prov/raw-file/default/model/prov-dm.html#term-ActivityAssociation</prov-dm>
        <category>qualified</category>
        <definition>An activity association is an assignment of responsibility to an agent for an activity, indicating that the agent had a role in the activity. It further allows for a plan to be specified, which is the plan intended by the agent to achieve some goals in the context of this activity.</definition>
        <rdfs:comment xml:lang="en">An instance of prov:Association provides additional descriptions about the binary prov:wasAssociatedWith relation from an prov:Activity to some prov:Agent that is responsible for it. For example, :baking prov:wasAssociatedWith :baker; prov:qualified [ a prov:Association; prov:agent :baker; :foo :bar ].</rdfs:comment>
        <prov-dm-constraints>http://dvcs.w3.org/hg/prov/raw-file/default/model/prov-dm-constraints.html#term-Association</prov-dm-constraints>
        <unqualifiedForm rdf:resource="http://www.w3.org/ns/prov#wasAssociatedWith"/>
    </owl:Class>
    


    <!-- http://www.w3.org/ns/prov#Attribution -->

    <owl:Class rdf:about="http://www.w3.org/ns/prov#Attribution">
        <rdfs:label>Attribution</rdfs:label>
        <rdfs:subClassOf rdf:resource="http://www.w3.org/ns/prov#AgentInvolvement"/>
        <definition>Attribution is the ascribing of an entity to an agent.</definition>
        <prov-dm>http://dvcs.w3.org/hg/prov/raw-file/default/model/prov-dm.html#term-attribution</prov-dm>
        <prov-n>http://dvcs.w3.org/hg/prov/raw-file/default/model/prov-n.html#expression-attribution</prov-n>
        <category>qualified</category>
        <rdfs:comment xml:lang="en">An instance of prov:Attribution provides additional descriptions about the binary prov:wasAttributedTo relation from an prov:Entity to some prov:Agent that is responsible for it. For example, :cake prov:wasAttributedTo :baker; prov:qualified [ a prov:Attribution; prov:entity :baker; :foo :bar ].</rdfs:comment>
        <prov-dm-constraints>http://dvcs.w3.org/hg/prov/raw-file/default/model/prov-dm-constraints.html#recod-attribution</prov-dm-constraints>
        <component>agents-responsibility</component>
        <unqualifiedForm rdf:resource="http://www.w3.org/ns/prov#wasAttributedTo"/>
    </owl:Class>
    


    <!-- http://www.w3.org/ns/prov#Bundle -->

    <owl:Class rdf:about="http://www.w3.org/ns/prov#Bundle">
        <rdfs:label>Bundle</rdfs:label>
        <rdfs:subClassOf rdf:resource="http://www.w3.org/ns/prov#Entity"/>
        <definition rdf:datatype="&xsd;anyURI">An account is any mechanism by which a set of provenance descriptions can be bundled up and named.</definition>
        <editorialNote xml:lang="en">Bundles expressed in PROV-O (i.e. RDF) may be modeled using:

:account1
   a prov:Bundle, sd:NamedGraph; 
   sd:name &lt;&gt;; 
   sd:graph [ a void:Dataset; void:dataDump &lt;&gt;; void:triples x ] .

Abstract accounts that are independent of location may be modeled using:

:account2
   a prov:Bundle, void:Dataset; 
   void:dataDump &lt;&gt;; 
    void:triples        x .


(sd : http://www.w3.org/ns/sparql-service-description#)
(void : http://rdfs.org/ns/void#)</editorialNote>
        <category>expanded</category>
        <prov-dm>http://dvcs.w3.org/hg/prov/raw-file/default/model/prov-dm.html#FurtherConsiderations</prov-dm>
        <prov-dm-constraints>http://dvcs.w3.org/hg/prov/raw-file/default/model/prov-dm-constraints.html#account-constraints</prov-dm-constraints>
        <rdfs:comment xml:lang="en">Note that there are kinds of accounts (e.g. handwritten letters, audio recordings, etc.) that are not expressed in PROV-O, but can be still be described by PROV-O.</rdfs:comment>
        <prov-n>http://dvcs.w3.org/hg/prov/raw-file/default/model/prov-n.html#account</prov-n>
    </owl:Class>
    


    <!-- http://www.w3.org/ns/prov#Collection -->

    <owl:Class rdf:about="http://www.w3.org/ns/prov#Collection">
        <rdfs:label xml:lang="en">Collection</rdfs:label>
        <rdfs:subClassOf rdf:resource="http://www.w3.org/ns/prov#Entity"/>
        <category>collections</category>
        <component>collections</component>
        <prov-dm>http://dvcs.w3.org/hg/prov/raw-file/default/model/prov-dm.html#term-collection</prov-dm>
        <definition xml:lang="en">A collection is an entity that provides a structure to some constituents, which are themselves entities. These constituents are said to be member of the collections.

A collection is a multiset of entities (it is a multiset, rather than a set, because it may not be possible to verify that two distinct entity identitifiers do not denote, in fact, the same entity).</definition>
        <editorialNote xml:lang="en">Note that although prov:Collection is defined, few other constructs in PROV-DM and PROV-O elaborate what it is or how to use it. Instead, they both elaborate one of its specializations, prov:Dictionary. Although some of the term names relating to prov:Dictionary may seem that they should also apply to prov:Collection, they are specific to prov:Dictionary. It is left to extensions of PROV-O to provide the terms relating to the insertion and removal of members of the more general class prov:Collection.</editorialNote>
    </owl:Class>
    


    <!-- http://www.w3.org/ns/prov#Communication -->

    <owl:Class rdf:about="http://www.w3.org/ns/prov#Communication">
        <rdfs:label>Communication</rdfs:label>
        <rdfs:subClassOf rdf:resource="http://www.w3.org/ns/prov#ActivityInvolvement"/>
        <category>qualified</category>
        <rdfs:comment xml:lang="en">An instance of prov:Communication provides additional descriptions about the binary prov:wasInformedBy relation from an informed prov:Activity to the prov:Activity that informed it. For example, :you_jumping_off_bridge prov:wasInformedBy :everyone_else_jumping_off_bridge; prov:qualifiedCommunication [ a prov:Communication; prov:entity :everyone_else_jumping_off_bridge; :foo :bar ].</rdfs:comment>
        <prov-dm-constraints>http://dvcs.w3.org/hg/prov/raw-file/default/model/prov-dm-constraints.html#term-Communication</prov-dm-constraints>
        <component>entities-activities</component>
        <prov-dm>http://dvcs.w3.org/hg/prov/raw-file/default/model/prov-dm.html#term-wasInformedBy</prov-dm>
        <prov-n>http://dvcs.w3.org/hg/prov/raw-file/default/model/prov-n.html#expression-wasInformedBy</prov-n>
        <definition>Communication is the exchange of an entity by two activities, one activity using the entity generated by the other.</definition>
        <unqualifiedForm rdf:resource="http://www.w3.org/ns/prov#wasInformedBy"/>
    </owl:Class>
    


    <!-- http://www.w3.org/ns/prov#CompleteCollection -->

    <owl:Class rdf:about="http://www.w3.org/ns/prov#CompleteCollection">
        <rdfs:label xml:lang="en">CompleteMembership</rdfs:label>
        <rdfs:subClassOf rdf:resource="http://www.w3.org/ns/prov#Collection"/>
        <category>collections</category>
        <rdfs:comment xml:lang="en">Indicates that no other member belongs to the collection, that is all the prov:member stated for this CompleteMembership constitutes all members of the collection.</rdfs:comment>
        <component xml:lang="en">collections</component>
    </owl:Class>
    


    <!-- http://www.w3.org/ns/prov#ContextualizedEntity -->

    <owl:Class rdf:about="http://www.w3.org/ns/prov#ContextualizedEntity">
        <rdfs:subClassOf rdf:resource="http://www.w3.org/ns/prov#Entity"/>
        <rdfs:comment>expanded</rdfs:comment>
        <prov-dm>http://dvcs.w3.org/hg/prov/raw-file/default/model/releases/ED-prov-dm-20120614/prov-dm.html#term-contextualization</prov-dm>
        <definition xml:lang="en">An entity that is a contextualization of another entity presents all aspects of the latter as per the latter&#39;s description in another bundle (referred to as remote bundle), and therefore constitutes a particular case of specialization of the latter entity.</definition>
    </owl:Class>
    


    <!-- http://www.w3.org/ns/prov#Delegation -->

    <owl:Class rdf:about="http://www.w3.org/ns/prov#Delegation">
        <rdfs:label>Delegation</rdfs:label>
        <rdfs:subClassOf rdf:resource="http://www.w3.org/ns/prov#AgentInvolvement"/>
        <category>qualified</category>
        <prov-n>http://dvcs.w3.org/hg/prov/raw-file/default/model/prov-n.html#expression-responsibility TODO</prov-n>
        <rdfs:comment xml:lang="en">An instance of prov:Delegation provides additional descriptions about the binary prov:actedOnBehalfOf relation from a performing prov:Agent to some prov:Agent for whom it was performed. For example, :mixing prov:wasAssociatedWith :toddler . :toddler prov:actedOnBehalfOf :mother; prov:qualifiedDelegation [ a prov:Delegation; prov:entity :mother; :foo :bar ].</rdfs:comment>
        <definition>Delegation is the assignment of authority and responsibility to an agent (by itself or by another agent) to carry out a specific activity as a delegate or representative, while the agent it acts on behalf of retains some responsibility for the outcome of the delegated work. </definition>
        <component>agents-responsibility</component>
        <prov-dm-constraints>http://dvcs.w3.org/hg/prov/raw-file/default/model/prov-dm-constraints.html#term-Responsibility TODO</prov-dm-constraints>
        <prov-dm>http://dvcs.w3.org/hg/prov/raw-file/default/model/prov-dm.html#term-delegation</prov-dm>
        <unqualifiedForm rdf:resource="http://www.w3.org/ns/prov#actedOnBehalfOf"/>
    </owl:Class>
    


    <!-- http://www.w3.org/ns/prov#Derivation -->

    <owl:Class rdf:about="http://www.w3.org/ns/prov#Derivation">
        <rdfs:label>Derivation</rdfs:label>
        <rdfs:subClassOf rdf:resource="http://www.w3.org/ns/prov#EntityInvolvement"/>
        <component>derivations</component>
        <rdfs:comment xml:lang="en">An instance of prov:Derivation provides additional descriptions about the binary prov:wasDerivedFrom relation from some prov:Entity to another prov:Entity. For example, :chewed_bubble_gum prov:wasDerivedFrom :unwrapped_bubble_gum; prov:qualified [ a prov:Derivation; prov:entity :unwrapped_bubble_gum; :foo :bar ].</rdfs:comment>
        <category>qualified</category>
        <prov-dm>http://dvcs.w3.org/hg/prov/raw-file/default/model/prov-dm.html#Derivation-Relation</prov-dm>
        <prov-dm-constraints>http://dvcs.w3.org/hg/prov/raw-file/default/model/prov-dm-constraints.html#Derivation-Relation</prov-dm-constraints>
        <prov-n>http://dvcs.w3.org/hg/prov/raw-file/default/model/prov-n.html#Derivation-Relation</prov-n>
        <definition>A derivation is a transformation of an entity into another, a construction of an entity into another, or an update of an entity, resulting in a new one.</definition>
        <unqualifiedForm rdf:resource="http://www.w3.org/ns/prov#wasDerivedFrom"/>
    </owl:Class>
    


    <!-- http://www.w3.org/ns/prov#Dictionary -->

    <owl:Class rdf:about="http://www.w3.org/ns/prov#Dictionary">
        <rdfs:label xml:lang="en">Dictionary</rdfs:label>
        <rdfs:subClassOf rdf:resource="http://www.w3.org/ns/prov#Collection"/>
        <prov-n>http://dvcs.w3.org/hg/prov/raw-file/default/model/prov-n.html#component6</prov-n>
        <prov-dm>http://dvcs.w3.org/hg/prov/raw-file/default/model/prov-dm.html#term-dictionary</prov-dm>
        <prov-dm-constraints>http://dvcs.w3.org/hg/prov/raw-file/default/model/prov-constraints.html#collection-constraints</prov-dm-constraints>
        <definition xml:lang="en">A dictionary is a collection whose members are indexed by keys.</definition>
        <rdfs:comment xml:lang="en">A given dictionary forms a given structure for its members. A different structure (obtained either by insertion or removal of members) constitutes a different dictionary.</rdfs:comment>
        <component>collections</component>
        <rdfs:comment xml:lang="en">PROV-DM defines a specific type of collection, a dictionary...</rdfs:comment>
        <rdfs:comment xml:lang="en">This concept allows for the provenance of the dictionary, but also of its constituents to be expressed. Such a notion of dictionary corresponds to a wide variety of concrete data structures, such as a maps or associative arrays.</rdfs:comment>
        <category>collections</category>
    </owl:Class>
    


    <!-- http://www.w3.org/ns/prov#DictionaryInvolvement -->

    <owl:Class rdf:about="http://www.w3.org/ns/prov#DictionaryInvolvement">
        <rdfs:subClassOf rdf:resource="http://www.w3.org/ns/prov#Involvement"/>
        <category>collections</category>
        <component>collections</component>
        <editorsDefinition xml:lang="en">prov:DictionaryInvolvement provides descriptions of any binary involvement between any instance and a prov:Dictionary. The property prov:dictionary is used to reference the object of the triple being described.</editorsDefinition>
    </owl:Class>
    


    <!-- http://www.w3.org/ns/prov#EmptyCollection -->

    <owl:Class rdf:about="http://www.w3.org/ns/prov#EmptyCollection">
        <rdfs:label xml:lang="en">Dictionary</rdfs:label>
        <rdfs:subClassOf rdf:resource="http://www.w3.org/ns/prov#Collection"/>
        <component>collections</component>
        <prov-dm>http://dvcs.w3.org/hg/prov/raw-file/default/model/prov-dm.html#term-dictionary</prov-dm>
        <category>collections</category>
        <definition xml:lang="en">An empty collection is a collection without members.</definition>
        <rdfs:comment xml:lang="en">An empty dictionary.</rdfs:comment>
    </owl:Class>
    


    <!-- http://www.w3.org/ns/prov#End -->

    <owl:Class rdf:about="http://www.w3.org/ns/prov#End">
        <rdfs:label>End</rdfs:label>
        <rdfs:subClassOf rdf:resource="http://www.w3.org/ns/prov#EntityInvolvement"/>
        <rdfs:subClassOf rdf:resource="http://www.w3.org/ns/prov#InstantaneousEvent"/>
        <prov-dm-constraints>http://dvcs.w3.org/hg/prov/raw-file/default/model/prov-dm-constraints.html#types-of-events</prov-dm-constraints>
        <prov-dm>http://dvcs.w3.org/hg/prov/raw-file/default/model/prov-dm.html#term-End</prov-dm>
        <prov-dm-constraints>http://dvcs.w3.org/hg/prov/raw-file/default/model/prov-dm-constraints.html#term-End</prov-dm-constraints>
        <category>qualified</category>
        <prov-n>http://dvcs.w3.org/hg/prov/raw-file/default/model/prov-n.html#expression-End</prov-n>
        <definition>An activity end event is the instantaneous event that marks the instant an activity ends.</definition>
        <rdfs:comment xml:lang="en">An instance of prov:End provides additional descriptions about the binary prov:wasEndedBy relation from some ended prov:Activity to an prov:Entity that ended it. For example, :ball_game prov:wasEndedBy :buzzer; prov:qualified [ a prov:Usage; prov:entity :buzzer; :foo :bar; prov:atTime &#39;2012-03-09T08:05:08-05:00&#39;^^xsd:dateTime ].</rdfs:comment>
        <component>entities-activities</component>
        <unqualifiedForm rdf:resource="http://www.w3.org/ns/prov#wasEndedBy"/>
    </owl:Class>
    


    <!-- http://www.w3.org/ns/prov#Entity -->

    <owl:Class rdf:about="http://www.w3.org/ns/prov#Entity">
        <rdfs:label>Entity</rdfs:label>
        <owl:disjointWith rdf:resource="http://www.w3.org/ns/prov#InstantaneousEvent"/>
        <prov-dm rdf:datatype="&xsd;anyURI">http://dvcs.w3.org/hg/prov/raw-file/default/model/prov-dm.html#section-entity-activity</prov-dm>
        <component>entities-activities</component>
        <definition xml:lang="en">An entity is a thing one wants to provide provenance for. For the purpose of this specification, things can be physical, digital, conceptual, or otherwise; things may be real or imaginary.</definition>
        <prov-dm-constraints>http://dvcs.w3.org/hg/prov/raw-file/default/model/prov-dm-constraints.html#term-Entity</prov-dm-constraints>
        <prov-n>http://dvcs.w3.org/hg/prov/raw-file/default/model/prov-n.html#expression-Entity</prov-n>
        <category>starting-point</category>
        <rdfs:comment xml:lang="en">An entity is a thing one wants to provide provenance for. For the purpose of this specification, things can be physical, digital, conceptual, or otherwise; things may be real or imaginary.</rdfs:comment>
    </owl:Class>
    


    <!-- http://www.w3.org/ns/prov#EntityInvolvement -->

    <owl:Class rdf:about="http://www.w3.org/ns/prov#EntityInvolvement">
        <rdfs:label>EntityInvolvement</rdfs:label>
        <rdfs:subClassOf rdf:resource="http://www.w3.org/ns/prov#Involvement"/>
        <rdfs:subClassOf>
            <owl:Restriction>
                <owl:onProperty rdf:resource="http://www.w3.org/ns/prov#activity"/>
                <owl:maxCardinality rdf:datatype="&xsd;nonNegativeInteger">0</owl:maxCardinality>
            </owl:Restriction>
        </rdfs:subClassOf>
        <category>qualified</category>
        <editorsDefinition xml:lang="en">prov:EntityInvolvement provides descriptions of any binary involvement between any instance and an prov:Entity. The property prov:entity is used to reference the object of the triple being described.</editorsDefinition>
        <rdfs:seeAlso rdf:resource="http://www.w3.org/ns/prov#entity"/>
    </owl:Class>
    


    <!-- http://www.w3.org/ns/prov#Generation -->

    <owl:Class rdf:about="http://www.w3.org/ns/prov#Generation">
        <rdfs:label>Generation</rdfs:label>
        <rdfs:subClassOf rdf:resource="http://www.w3.org/ns/prov#ActivityInvolvement"/>
        <rdfs:subClassOf rdf:resource="http://www.w3.org/ns/prov#InstantaneousEvent"/>
        <prov-dm-constraints>http://dvcs.w3.org/hg/prov/raw-file/default/model/prov-dm-constraints.html#term-Generation</prov-dm-constraints>
        <prov-n>http://dvcs.w3.org/hg/prov/raw-file/default/model/prov-n.html#expression-Generation</prov-n>
        <rdfs:comment xml:lang="en">An instance of prov:Generation provides additional descriptions about the binary prov:wasGeneratedBy relation from a generated prov:Entity to the prov:Activity that generated it. For example, :cake prov:wasGeneratedBy :baking; prov:qualifiedGeneration [ a prov:Generation; prov:activity :baking; :foo :bar ].</rdfs:comment>
        <prov-dm-constraints>http://dvcs.w3.org/hg/prov/raw-file/default/model/prov-dm-constraints.html#types-of-events</prov-dm-constraints>
        <category>qualified</category>
        <prov-dm>http://dvcs.w3.org/hg/prov/raw-file/default/model/prov-dm.html#term-Generation</prov-dm>
        <definition>An entity generation event is the instantaneous event that marks the final instant of an entity&#39;s creation timespan, after which it is no longer available for use.</definition>
        <component>entities-activities</component>
        <unqualifiedForm rdf:resource="http://www.w3.org/ns/prov#wasGeneratedBy"/>
    </owl:Class>
    


    <!-- http://www.w3.org/ns/prov#Insertion -->

    <owl:Class rdf:about="http://www.w3.org/ns/prov#Insertion">
        <rdfs:label>Insertion</rdfs:label>
        <rdfs:subClassOf rdf:resource="http://www.w3.org/ns/prov#DictionaryInvolvement"/>
        <definition>Insertion is a derivation that transforms a dictionary into another, by insertion of one or more key-value pairs.</definition>
        <rdfs:comment xml:lang="en">Insertion is a derivation that transforms a dictionary into another, by insertion of one or more key-value pairs.</rdfs:comment>
        <prov-dm>http://dvcs.w3.org/hg/prov/raw-file/default/model/prov-dm.html#term-collection-insertion</prov-dm>
        <prov-n>http://dvcs.w3.org/hg/prov/raw-file/default/model/prov-n.html#expression-collection-insertion</prov-n>
        <component>collections</component>
        <prov-dm-constraints>http://dvcs.w3.org/hg/prov/raw-file/default/model/prov-dm-constraints.html#term-Collection</prov-dm-constraints>
        <category>collections</category>
        <unqualifiedForm rdf:resource="http://www.w3.org/ns/prov#derivedByInsertionFrom"/>
    </owl:Class>
    


    <!-- http://www.w3.org/ns/prov#InstantaneousEvent -->

    <owl:Class rdf:about="http://www.w3.org/ns/prov#InstantaneousEvent">
        <rdfs:label>InstantaneousEvent</rdfs:label>
        <prov-n></prov-n>
        <component>entities-activities</component>
        <prov-dm></prov-dm>
        <definition>An instantaneous event, or event for short, happens in the world and marks a change in the world, in its activities and in its entities. The term &#39;event&#39; is commonly used in process algebra with a similar meaning. Events represent communications or interactions; they are assumed to be atomic and instantaneous.</definition>
        <rdfs:comment xml:lang="en">An instantaneous event, or event for short, happens in the world and marks a change in the world, in its activities and in its entities. The term &#39;event&#39; is commonly used in process algebra with a similar meaning. Events represent communications or interactions; they are assumed to be atomic and instantaneous.</rdfs:comment>
        <category>qualified</category>
        <prov-dm-constraints>http://dvcs.w3.org/hg/prov/raw-file/default/model/prov-constraints.html#event-ordering</prov-dm-constraints>
    </owl:Class>
    


    <!-- http://www.w3.org/ns/prov#Invalidation -->

    <owl:Class rdf:about="http://www.w3.org/ns/prov#Invalidation">
        <rdfs:subClassOf rdf:resource="http://www.w3.org/ns/prov#ActivityInvolvement"/>
        <rdfs:subClassOf rdf:resource="http://www.w3.org/ns/prov#InstantaneousEvent"/>
        <prov-n>http://dvcs.w3.org/hg/prov/raw-file/default/model/prov-n.html#expression-Invalidation</prov-n>
        <component>entities-activities</component>
        <category>qualified</category>
        <prov-dm>http://dvcs.w3.org/hg/prov/raw-file/default/model/prov-dm.html#term-Invalidation</prov-dm>
        <prov-dm-constraints>http://dvcs.w3.org/hg/prov/raw-file/default/model/prov-dm-constraints.html#dfn-invalidation-event</prov-dm-constraints>
        <definition>Invalidation is the start of the destruction, cessation, or expiry of an existing entity by an activity. The entity is no longer available for use after invalidation. Any generation or usage of an entity precedes its invalidation.</definition>
    </owl:Class>
    


    <!-- http://www.w3.org/ns/prov#Involvement -->

    <owl:Class rdf:about="http://www.w3.org/ns/prov#Involvement">
        <rdfs:label>Involvement</rdfs:label>
        <rdfs:comment xml:lang="en">Any resource that involved an prov:Activity, prov:Entity, or prov:Agent can qualify its involvement by also referencing an instance of prov:Involvement. Instances of prov:Involvement reference the involved Activity, Entity, or Agent (using prov:activity, prov:entity, or prov:agent, respectively) and may be described with any kind of attributes, including user-defined attributes and those provided by PROV (prov:hadRole, prov:hadPlan, prov:atTime, prov:hadLocation). A description (via prov:Involvement) of the binary involvement implies the assertion of the binary involvement.</rdfs:comment>
        <editorialNote>For simplicity, the hierarchy &#39;stops&#39; at the primary resources (Activity, Entity, Agent). Distinctions beyond the type of object involved are not necessary in PROV-O, but may be established by others.</editorialNote>
        <category>qualified</category>
        <unqualifiedForm rdf:resource="http://www.w3.org/ns/prov#involved"/>
    </owl:Class>
    


    <!-- http://www.w3.org/ns/prov#KeyValuePair -->

    <owl:Class rdf:about="http://www.w3.org/ns/prov#KeyValuePair">
        <rdfs:subClassOf rdf:resource="http://www.w3.org/ns/prov#Entity"/>
        <rdfs:comment xml:lang="en">A key-value pair. Part of a prov:Dictionary through prov:Membership. The key is any RDF Literal, the value is a prov:Entity.</rdfs:comment>
        <category>collections</category>
    </owl:Class>
    


    <!-- http://www.w3.org/ns/prov#Location -->

    <owl:Class rdf:about="http://www.w3.org/ns/prov#Location">
        <rdfs:label>Location</rdfs:label>
        <definition>A location can be an identifiable geographic place (ISO 19112), but it can also be a non-geographic place such as a directory, row, or column. As such, there are numerous ways in which location can be expressed, such as by a coordinate, address, landmark, and so forth.</definition>
        <prov-n></prov-n>
        <category>expanded</category>
        <prov-dm-constraints></prov-dm-constraints>
        <rdfs:comment xml:lang="en">A location can be an identifiable geographic place (ISO 19112), but it can also be a non-geographic place such as a directory, row, or column. As such, there are numerous ways in which location can be expressed, such as by a coordinate, address, landmark, and so forth.</rdfs:comment>
        <prov-dm>http://dvcs.w3.org/hg/prov/raw-file/default/model/prov-dm.html#term-attribute-location</prov-dm>
        <rdfs:seeAlso rdf:resource="http://www.w3.org/ns/prov#hadLocation"/>
    </owl:Class>
    


    <!-- http://www.w3.org/ns/prov#Membership -->

    <owl:Class rdf:about="http://www.w3.org/ns/prov#Membership">
        <rdfs:subClassOf rdf:resource="http://www.w3.org/ns/prov#EntityInvolvement"/>
        <editorsDefinition xml:lang="en">An optional set of descriptions about the membership of KeyValuePairs in a prov:Dictionary.</editorsDefinition>
        <rdfs:comment xml:lang="en">The descriptions on this Membership applies to the memberships of all KeyValuePairs cited by prov:pair.</rdfs:comment>
        <category>collections</category>
        <component>collections</component>
        <unqualifiedForm rdf:resource="http://www.w3.org/ns/prov#hadMember"/>
    </owl:Class>
    


    <!-- http://www.w3.org/ns/prov#Organization -->

    <owl:Class rdf:about="http://www.w3.org/ns/prov#Organization">
        <rdfs:label>Organization</rdfs:label>
        <rdfs:subClassOf rdf:resource="http://www.w3.org/ns/prov#Agent"/>
        <definition>Agents of type Organization are social institutions such as companies, societies etc.</definition>
        <prov-dm-constraints></prov-dm-constraints>
        <rdfs:comment xml:lang="en">Agents of type Organization are social institutions such as companies, societies etc.</rdfs:comment>
        <category>expanded</category>
        <prov-n>http://dvcs.w3.org/hg/prov/raw-file/default/model/prov-n.html#expression-types</prov-n>
        <component>agents-responsibility</component>
        <prov-dm>http://dvcs.w3.org/hg/prov/raw-file/default/model/prov-dm.html#term-Agent</prov-dm>
    </owl:Class>
    


    <!-- http://www.w3.org/ns/prov#Person -->

    <owl:Class rdf:about="http://www.w3.org/ns/prov#Person">
        <rdfs:label>Person</rdfs:label>
        <rdfs:subClassOf rdf:resource="http://www.w3.org/ns/prov#Agent"/>
        <category>expanded</category>
        <prov-n>http://dvcs.w3.org/hg/prov/raw-file/default/model/prov-n.html#expression-types</prov-n>
        <prov-dm>http://dvcs.w3.org/hg/prov/raw-file/default/model/prov-dm.html#term-Agent</prov-dm>
        <component>agents-responsibility</component>
        <definition>Agents of type Person are people.</definition>
        <prov-dm-constraints></prov-dm-constraints>
        <rdfs:comment xml:lang="en">Agents of type Person are people.</rdfs:comment>
    </owl:Class>
    


    <!-- http://www.w3.org/ns/prov#Plan -->

    <owl:Class rdf:about="http://www.w3.org/ns/prov#Plan">
        <rdfs:label>Plan</rdfs:label>
        <rdfs:subClassOf rdf:resource="http://www.w3.org/ns/prov#Entity"/>
        <prov-dm-constraints>http://dvcs.w3.org/hg/prov/raw-file/default/model/prov-dm-constraints.html#term-Association</prov-dm-constraints>
        <definition>A plan is an entity that represents a set of actions or steps intended by one or more agents to achieve some goals.</definition>
        <rdfs:comment xml:lang="en">There exist no prescriptive requirement on the nature of plans, their representation, the actions or steps they consist of, or their intended goals. Since plans may evolve over time, it may become necessary to track their provenance, so plans themselves are entities. Representing the plan explicitly in the provenance can be useful for various tasks: for example, to validate the execution as represented in the provenance record, to manage expectation failures, or to provide explanations.</rdfs:comment>
        <prov-n>http://dvcs.w3.org/hg/prov/raw-file/default/model/prov-n.html#expression-Association</prov-n>
        <category>qualified</category>
        <prov-dm>http://www.w3.org/TR/prov-dm/#association.plan</prov-dm>
        <component>agents-responsibility</component>
    </owl:Class>
    


    <!-- http://www.w3.org/ns/prov#ProvenanceService -->

    <owl:Class rdf:about="http://www.w3.org/ns/prov#ProvenanceService">
        <rdfs:subClassOf rdf:resource="http://www.w3.org/ns/prov#SoftwareAgent"/>
        <category>access-and-query</category>
        <rdfs:comment>Class for a service described by a provenance service description.</rdfs:comment>
        <prov-aq>http://dvcs.w3.org/hg/prov/raw-file/tip/paq/prov-aq.html#todo</prov-aq>
    </owl:Class>
    


    <!-- http://www.w3.org/ns/prov#Quotation -->

    <owl:Class rdf:about="http://www.w3.org/ns/prov#Quotation">
        <rdfs:label>Quotation</rdfs:label>
        <rdfs:subClassOf rdf:resource="http://www.w3.org/ns/prov#EntityInvolvement"/>
        <definition>A quotation is the repeat of (some or all of) an entity, such as text or image, by someone other than its original author.</definition>
        <component>derivations</component>
        <category>qualified</category>
        <rdfs:comment xml:lang="en">An instance of prov:Quotation provides additional descriptions about the binary prov:wasQuotedFrom relation from some prov:Entity to another prov:Entity. For example, :here_is_looking_at_you_kid prov:wasQuotedFrom :casablanca_script; prov:qualified [ a prov:Quotation; prov:entity :casablanca_script; :foo :bar ].</rdfs:comment>
        <prov-dm>http://dvcs.w3.org/hg/prov/raw-file/default/model/prov-dm.html#term-quotation</prov-dm>
        <prov-dm-constraints>http://dvcs.w3.org/hg/prov/raw-file/default/model/prov-dm-constraints.html#term-quotation</prov-dm-constraints>
        <prov-n>http://dvcs.w3.org/hg/prov/raw-file/default/model/prov-n.html#expression-quotation</prov-n>
        <unqualifiedForm rdf:resource="http://www.w3.org/ns/prov#wasQuotedFrom"/>
    </owl:Class>
    


    <!-- http://www.w3.org/ns/prov#Removal -->

    <owl:Class rdf:about="http://www.w3.org/ns/prov#Removal">
        <rdfs:label>Removal</rdfs:label>
        <rdfs:subClassOf rdf:resource="http://www.w3.org/ns/prov#DictionaryInvolvement"/>
        <category>collections</category>
        <prov-dm-constraints>http://dvcs.w3.org/hg/prov/raw-file/default/model/prov-dm-constraints.html#term-Collection</prov-dm-constraints>
        <definition>Removal is a derivation that transforms a dictionary into another, by removing one or more key-value pairs.</definition>
        <rdfs:comment xml:lang="en">Removal is a derivation that transforms a dictionary into another, by removing one or more key-value pairs.</rdfs:comment>
        <prov-n>http://dvcs.w3.org/hg/prov/raw-file/default/model/prov-n.html#expression-collection-removal</prov-n>
        <prov-dm>http://dvcs.w3.org/hg/prov/raw-file/default/model/prov-dm.html#term-collection-removal</prov-dm>
        <component>collections</component>
        <unqualifiedForm rdf:resource="http://www.w3.org/ns/prov#derivedByRemovalFrom"/>
    </owl:Class>
    


    <!-- http://www.w3.org/ns/prov#Revision -->

    <owl:Class rdf:about="http://www.w3.org/ns/prov#Revision">
        <rdfs:label>Revision</rdfs:label>
        <rdfs:subClassOf rdf:resource="http://www.w3.org/ns/prov#EntityInvolvement"/>
        <prov-dm-constraints>http://dvcs.w3.org/hg/prov/raw-file/default/model/prov-dm-constraints.html#term-Revision</prov-dm-constraints>
        <component>derivations</component>
        <category>qualified</category>
        <definition>A revision is a derivation that revises an entity into a revised version.</definition>
        <rdfs:comment xml:lang="en">An instance of prov:Revision provides additional descriptions about the binary prov:wasRevisionOf relation from some prov:Entity to another prov:Entity. For example, :draft_2 prov:wasRevisionOf :draft_1; prov:qualified [ a prov:Source; prov:entity :draft_1; :foo :bar ].</rdfs:comment>
        <prov-n>http://dvcs.w3.org/hg/prov/raw-file/default/model/prov-n.html#expression-Revision</prov-n>
        <prov-dm>http://dvcs.w3.org/hg/prov/raw-file/default/model/prov-dm.html#term-Revision</prov-dm>
        <unqualifiedForm rdf:resource="http://www.w3.org/ns/prov#wasRevisionOf"/>
    </owl:Class>
    


    <!-- http://www.w3.org/ns/prov#Role -->

    <owl:Class rdf:about="http://www.w3.org/ns/prov#Role">
        <rdfs:label>Role</rdfs:label>
        <category>qualified</category>
        <prov-n></prov-n>
        <prov-dm>http://dvcs.w3.org/hg/prov/raw-file/default/model/prov-dm.html#term-attribute-role</prov-dm>
        <prov-dm-constraints></prov-dm-constraints>
        <definition>A Role is the function of an entity with respect to an activity, in the context of a usage, generation, association, start, and end.</definition>
        <rdfs:comment xml:lang="en">A Role is the function of an entity with respect to an activity, in the context of a usage, generation, association, start, and end.</rdfs:comment>
        <component>agents-responsibility</component>
        <rdfs:seeAlso rdf:resource="http://www.w3.org/ns/prov#hadRole"/>
    </owl:Class>
    


    <!-- http://www.w3.org/ns/prov#SoftwareAgent -->

    <owl:Class rdf:about="http://www.w3.org/ns/prov#SoftwareAgent">
        <rdfs:label>SoftwareAgent</rdfs:label>
        <rdfs:subClassOf rdf:resource="http://www.w3.org/ns/prov#Agent"/>
        <prov-n>http://dvcs.w3.org/hg/prov/raw-file/default/model/prov-n.html#expression-types</prov-n>
        <prov-dm>http://dvcs.w3.org/hg/prov/raw-file/default/model/prov-dm.html#term-Agent</prov-dm>
        <prov-dm-constraints></prov-dm-constraints>
        <rdfs:comment xml:lang="en">A software agent is running software.</rdfs:comment>
        <component>agents-responsibility</component>
        <category>expanded</category>
        <definition>A software agent is running software.</definition>
    </owl:Class>
    


    <!-- http://www.w3.org/ns/prov#Source -->

    <owl:Class rdf:about="http://www.w3.org/ns/prov#Source">
        <rdfs:label>Source</rdfs:label>
        <rdfs:subClassOf rdf:resource="http://www.w3.org/ns/prov#EntityInvolvement"/>
        <prov-n>http://dvcs.w3.org/hg/prov/raw-file/default/model/prov-n.html#expression-original-source</prov-n>
        <definition>An original source refers to the source material that is closest to the person, information, period, or idea being studied.</definition>
        <prov-dm-constraints>http://dvcs.w3.org/hg/prov/raw-file/default/model/prov-dm-constraints.html#term-orignal-source</prov-dm-constraints>
        <rdfs:comment xml:lang="en">An instance of prov:Source provides additional descriptions about the binary prov:hadOriginalSource relation from some prov:Entity to another prov:Entity. For example, :blog prov:hadOriginalSource :newsArticle; prov:qualified [ a prov:Source; prov:entity :newsArticle; :foo :bar ].</rdfs:comment>
        <category>qualified</category>
        <component>derivations</component>
        <prov-dm>http://dvcs.w3.org/hg/prov/raw-file/default/model/prov-dm.html#term-original-source</prov-dm>
        <unqualifiedForm rdf:resource="http://www.w3.org/ns/prov#hadPrimarySource"/>
    </owl:Class>
    


    <!-- http://www.w3.org/ns/prov#Start -->

    <owl:Class rdf:about="http://www.w3.org/ns/prov#Start">
        <rdfs:label>Start</rdfs:label>
        <rdfs:subClassOf rdf:resource="http://www.w3.org/ns/prov#EntityInvolvement"/>
        <rdfs:subClassOf rdf:resource="http://www.w3.org/ns/prov#InstantaneousEvent"/>
        <definition>An activity start event is the instantaneous event that marks the instant an activity starts.</definition>
        <prov-dm-constraints>http://dvcs.w3.org/hg/prov/raw-file/default/model/prov-dm-constraints.html#types-of-events</prov-dm-constraints>
        <component>entities-activities</component>
        <rdfs:comment xml:lang="en">An instance of prov:Start provides additional descriptions about the binary prov:wasStartedBy relation from some started prov:Activity to an prov:Entity that started it. For example, :foot_race prov:wasStartedBy :bang; prov:qualified [ a prov:Usage; prov:entity :bang; :foo :bar; prov:atTime &#39;2012-03-09T08:05:08-05:00&#39;^^xsd:dateTime ].</rdfs:comment>
        <category>qualified</category>
        <prov-n>http://dvcs.w3.org/hg/prov/raw-file/default/model/prov-n.html#expression-Start</prov-n>
        <prov-dm-constraints>http://dvcs.w3.org/hg/prov/raw-file/default/model/prov-dm-constraints.html#term-Start</prov-dm-constraints>
        <prov-dm>http://dvcs.w3.org/hg/prov/raw-file/default/model/prov-dm.html#term-Start</prov-dm>
        <unqualifiedForm rdf:resource="http://www.w3.org/ns/prov#wasStartedBy"/>
    </owl:Class>
    


    <!-- http://www.w3.org/ns/prov#Trace -->

    <owl:Class rdf:about="http://www.w3.org/ns/prov#Trace">
        <rdfs:label>Trace</rdfs:label>
        <rdfs:subClassOf rdf:resource="http://www.w3.org/ns/prov#EntityInvolvement"/>
        <definition>Traceability is the ability to link back an entity to another by means of derivation or responsibility relations, possibly repeatedly traversed.</definition>
        <rdfs:comment xml:lang="en">An instance of prov:Trace provides additional descriptions about the binary prov:tracedTo relation from some prov:Entity to some other prov:Element. For example, :stomach_ache prov:tracedTo :spoon; prov:qualified [ a prov:Trace; prov:entity :spoon; :foo :bar ].</rdfs:comment>
        <prov-dm>http://dvcs.w3.org/hg/prov/raw-file/default/model/prov-dm.html#term-traceability</prov-dm>
        <category>qualified</category>
        <prov-dm-constraints>http://dvcs.w3.org/hg/prov/raw-file/default/model/prov-dm-constraints.html#term-traceability</prov-dm-constraints>
        <prov-n>http://dvcs.w3.org/hg/prov/raw-file/default/model/prov-n.html#expression-traceability</prov-n>
        <component>derivations</component>
        <unqualifiedForm rdf:resource="http://www.w3.org/ns/prov#tracedTo"/>
    </owl:Class>
    


    <!-- http://www.w3.org/ns/prov#Usage -->

    <owl:Class rdf:about="http://www.w3.org/ns/prov#Usage">
        <rdfs:label>Usage</rdfs:label>
        <rdfs:subClassOf rdf:resource="http://www.w3.org/ns/prov#EntityInvolvement"/>
        <rdfs:subClassOf rdf:resource="http://www.w3.org/ns/prov#InstantaneousEvent"/>
        <prov-n>http://dvcs.w3.org/hg/prov/raw-file/default/model/prov-n.html#expression-Usage</prov-n>
        <definition>A usage is an instantaneous world event: an activity beginning to consume an entity. Before this event, the activity had not begun to consume or use to this entity.</definition>
        <category>qualified</category>
        <component>entities-activities</component>
        <prov-dm-constraints>http://dvcs.w3.org/hg/prov/raw-file/default/model/prov-dm-constraints.html#types-of-events</prov-dm-constraints>
        <prov-dm>http://dvcs.w3.org/hg/prov/raw-file/default/model/prov-dm.html#term-Usage</prov-dm>
        <prov-dm-constraints>http://dvcs.w3.org/hg/prov/raw-file/default/model/prov-dm-constraints.html#term-Usage</prov-dm-constraints>
        <rdfs:comment xml:lang="en">An instance of prov:Usage provides additional descriptions about the binary prov:used relation from some prov:Activity to an prov:Entity that it used. For example, :keynote prov:used :podium; prov:qualified [ a prov:Usage; prov:entity :podium; :foo :bar ].</rdfs:comment>
        <unqualifiedForm rdf:resource="http://www.w3.org/ns/prov#used"/>
    </owl:Class>
</rdf:RDF>



<!-- Generated by the OWL API (version 3.1.0.20069) http://owlapi.sourceforge.net -->

