@prefix owl:     <http://www.w3.org/2002/07/owl#> .
@prefix rdfs:    <http://www.w3.org/2000/01/rdf-schema#> .
@prefix time:    <http://www.w3.org/2006/time#> .
@prefix dcterms: <http://purl.org/dc/terms/> .
@prefix prov:    <http://www.w3.org/ns/prov-o/> .

prov:qualified
   a owl:ObjectProperty;
   rdfs:label "qualified";
   rdfs:comment "OBE(no need for subproperties; it's handled by the type of the object): The superproperty of qualifiedUsage, qualifiedGeneration, qualifiedParticipation, and qualifiedControl that associates some Activity or Entity with another Activity or Entity.";
   rdfs:domain [ owl:unionOf ( prov:Activity prov:Entity ) ];
   rdfs:range prov:Involvement;
.

prov:Involvement
   a owl:Class;
   rdfs:label "Involvement";
.

prov:EntityInvolvement
   a owl:Class;
   rdfs:label "EntityInvolvement";
   rdfs:subClassOf prov:Involvement;
   rdfs:subClassOf [
       owl:onProperty prov:entity;
       owl:minCardinality 1;
   ];
.

prov:Generation rdfs:subClassOf prov:EntityInvolvement .
prov:Used rdfs:subClassOf prov:EntityInvolvement .
prov:Association 
   rdfs:subClassOf prov:EntityInvolvement; 
   rdfs:subClassOf [ 
      owl:onProperty prov:entity; 
      owl:allValuesFrom prov:Agent 
   ];
.

prov:ActivityInvolvement
   a owl:Class;
   rdfs:label "ActivityInvolvement";
   rdfs:subClassOf prov:Involvement;
   rdfs:subClassOf [
       owl:onProperty prov:activity;
       owl:minCardinality 1;
   ];
.

prov:Inform
   a owl:Class;
   rdfs:comment "The Qualified form of the binary relation prov:wasInformedBy";
   rdfs:subClassOf prov:ActivityInvolvement;
   rdfs:seeAlso prov:wasInformedBy;
.

prov:entity
   a owl:ObjectProperty;
   rdfs:label "entity";
   rdfs:comment "The Entity whose involvement (PE's used, hadParticipant, wasControlledBy, or generation) is being qualified.";
   rdfs:comment "This is effectively the rdf:object or owl:AnnotationTarget of the triple being reified.";
   rdfs:domain prov:EntityInvolvement;
   rdfs:range  prov:Entity;
.

prov:activity
   a owl:ObjectProperty;
   rdfs:label "entity";
   rdfs:comment "The Activity whose involvement is being qualified.";
   rdfs:comment "This is effectively the rdf:object or owl:AnnotationTarget of the triple being reified.";
   rdfs:domain prov:ActivityInvolvement;
   rdfs:range  prov:Activity;
.
