@prefix rdf:     <http://www.w3.org/1999/02/22-rdf-syntax-ns#> .
@prefix rdfs:    <http://www.w3.org/2000/01/rdf-schema#> .
@prefix owl:     <http://www.w3.org/2002/07/owl#> .
@prefix rdfs:    <http://www.w3.org/2000/01/rdf-schema#> .
@prefix time:    <http://www.w3.org/2006/time#> .
@prefix dcterms: <http://purl.org/dc/terms/> .
@prefix prov:    <http://www.w3.org/ns/prov-o/> .

prov:Quote
   a owl:Class;
   rdfs:label "Quote";
   rdfs:comment "A value quoted from a previous, usually larger entity.";
   rdfs:seeAlso <http://www.w3.org/TR/2011/WD-prov-dm-20111018/#quotation>,
                <http://www.w3.org/TR/2011/WD-prov-dm-20111018/#attribution>;

   rdfs:subClassOf prov:Entity;

   rdfs:comment "To be a Quote, it must have come from some previous entity.";
   rdfs:subClassOf [
      a owl:Restriction;
      owl:onProperty prov:wasQuotedFrom;
      owl:minCardinality 1;
   ];
   rdfs:comment "If the quote is some string, then the string can be provided using rdf:value.";
   rdfs:subClassOf [
      a owl:Restriction;
      owl:onProperty rdf:value;
      owl:cardinality 1;
   ];
.

prov:wasQuotedFrom 
   rdfs:seeAlso <http://www.w3.org/TR/2011/WD-prov-dm-20111018/#attribution>,
                <http://www.w3.org/TR/2011/WD-prov-dm-20111018/#quotation>,
                <http://www.w3.org/2011/prov/track/issues/151>;
   rdfs:label "wasQuotedFrom";
   rdfs:domain prov:Quote;
   rdfs:subPropertyOf prov:wasDerivedFrom;
   rdfs:range  prov:QuotedEntity;
.

prov:Quotivity
   a owl:Class;
   rdfs:label   "Quotation";
   rdfs:comment "Qualification about how a Quote was a quote of its source.";
   rdfs:seeAlso <http://www.w3.org/TR/2011/WD-prov-dm-20111018/#quotation>;
   rdfs:subClassOf prov:Activity;
   rdfs:comment "An optional prov:hadQuoter can cite the Agent responsible for quoting the previous Entity.";
   rdfs:subClassOf [
      a owl:Restriction;
      owl:onProperty prov:hadQuoter;
      owl:minCardinality 0;
   ];
   rdfs:comment "At least one prov:used must cite the Entity that was quoted.";
   rdfs:subClassOf [
      a owl:Restriction;
      owl:onProperty prov:used;
      owl:minQualifiedCardinality 1;
      owl:onClass prov:QuotedEntity;
   ];
   rdfs:comment "An optional prov:hadQuotee can cite the Agent responsible for the quoted Entity.";
   rdfs:subClassOf [
      a owl:Restriction;
      owl:onProperty prov:hasQuotee;
      owl:minCardinality 0;
   ];
.

prov:hadQuoter
   a owl:ObjectProperty;
   rdfs:label   "hasQuoter";
   rdfs:comment "The agent that cited the source of the quote.";
   rdfs:comment "an agent who is doing the quoting";
   rdfs:subPropertyOf prov:wasControlledBy;
   rdfs:domain prov:Quotivity;
   rdfs:range  prov:Agent;
.

prov:hasQuotee 
   a owl:ObjectProperty;
   rdfs:label   "hasQuotee";
   rdfs:comment "The agent associated with the source of the quote.";
   rdfs:comment "prov:involved is a superproperty of used, wasControlledBy, and hadParticipant. The quoted author did not participate, but _is_ indirectly involved.";
   rdfs:comment "the agent that is quoted";
   rdfs:subPropertyOf prov:involved;
   rdfs:domain prov:Quotivity;
   rdfs:range  prov:Agent;
.

 prov:wasAttributedTo
   a owl:ObjectProperty;
   rdfs:label "wasAttributedTo";
   rdfs:comment "Part of quotation-implication constraint in DM.";
   rdfs:domain prov:Entity;
   rdfs:range  prov:Agent;
.
